prove completeness

Completeness.v
@@ -1,4 +1,5 @@
-From SymCoreTheory Require Import SymCore ConCore.
+From SymCoreTheory Require Import SymCore ConCore BranchLaws CostLaws.
+From Stdlib Require Import Bool.Bool Arith.Wf_nat.
 From Stdlib Require Import Strings.String.
 From Stdlib Require Import Lists.List.
 From Stdlib Require Import Lia.
@@ -329,3 +330,1652 @@ Section AppliedCaseWithBranchScrutinee.
 End AppliedCaseWithBranchScrutinee.
 
 End Completeness.
+
+Section CostBasics.
+Context {sorts : SymCoreSorts} {solver : SymCoreSolver} {laws : SymFCCostLaws}.
+
+Lemma contains_env_k_sym_free : forall σ S k Γs Γc,
+  contains_env_k σ S k Γs Γc -> sym_free_env S Γs.
+Proof.
+  intros σ S k Γs Γc H.
+  exact (proj1 (contains_env_sym_free σ S Γs Γc (contains_env_k_erase _ _ _ _ _ H))).
+Qed.
+
+Lemma contains_env_k_concrete : forall σ S k Γs Γc,
+  contains_env_k σ S k Γs Γc -> concrete_env Γc.
+Proof.
+  intros σ S k Γs Γc H.
+  exact (contains_env_concrete σ S Γs Γc (contains_env_k_erase _ _ _ _ _ H)).
+Qed.
+
+Lemma contains_env_k_lookup : forall σ S k Γs Γc x Γs' es,
+  contains_env_k σ S k Γs Γc ->
+  lookup_env Γs x = Some (Γs', es) ->
+  exists Γc' ec k1 k2,
+    lookup_env Γc x = Some (Γc', ec) /\ contains_env_k σ S k1 Γs' Γc' /\
+    contains_k σ S k2 es ec /\ k1 <= k /\ k2 <= k.
+Proof.
+  intros σ S k Γs Γc x Γs' es H. revert Γs' es.
+  induction H as [| kenv ke krest y Γ1 Γ2 e1 e2 r1 r2 Hy Henv _ He Hc Hrest IH];
+    intros Γs' es Hl; simpl in Hl; [discriminate |].
+  simpl. destruct (string_dec x y).
+  - injection Hl as <- <-. exists Γ2, e2, kenv, ke. repeat split; try assumption; lia.
+  - destruct (IH Γs' es Hl) as [Γc' [ec [k1 [k2 [Hlc [H1 [H2 [Hk1 Hk2]]]]]]]].
+    exists Γc', ec, k1, k2. repeat split; try assumption; lia.
+Qed.
+
+Lemma delay_contains_k : forall σ S kenv k Γs Γc es ec,
+  contains_env_k σ S kenv Γs Γc ->
+  contains_k σ S k es ec ->
+  exists k', k' <= 1 + kenv + k /\ contains_k σ S k' (delay Γs es) (delay Γc ec).
+Proof.
+  intros σ S kenv k Γs Γc es ec Henv Hc.
+  destruct (is_thunk es) eqn:Hs; destruct (is_thunk ec) eqn:Hcc.
+  - rewrite (delay_thunk Γs es Hs), (delay_thunk Γc ec Hcc). exists k. split; [lia | exact Hc].
+  - exfalso. destruct es; try discriminate Hs.
+    inversion Hc; subst; simpl in *; congruence.
+  - rewrite (delay_not_thunk Γs es Hs), (delay_thunk Γc ec Hcc).
+    exists (1 + kenv + k). split; [lia |]. exact (ContK_Thunk_Outer σ S kenv k Γs Γc es ec Henv Hc Hcc).
+  - rewrite (delay_not_thunk Γs es Hs), (delay_not_thunk Γc ec Hcc).
+    exists (kenv + k). split; [lia |]. apply ContK_Thunk; assumption.
+Qed.
+
+Lemma delay_map_contains_k : forall σ S kenv Γs Γc ks args_s args_c,
+  contains_env_k σ S kenv Γs Γc ->
+  Forall3 (contains_k σ S) ks args_s args_c ->
+  exists ks', list_sum ks' <= length ks * (1 + kenv) + list_sum ks /\
+    Forall3 (contains_k σ S) ks' (map (delay Γs) args_s) (map (delay Γc) args_c).
+Proof.
+  intros σ S kenv Γs Γc ks args_s args_c Henv HF.
+  induction HF as [| k a_s a_c ks l1 l2 Ha _ IH].
+  - exists nil. split; [simpl; lia | constructor].
+  - destruct IH as [ks' [Hs HF']].
+    destruct (delay_contains_k σ S kenv k Γs Γc a_s a_c Henv Ha) as [k' [Hk' Hd]].
+    exists (k' :: ks'). split; [simpl in *; lia | constructor; assumption].
+Qed.
+
+Lemma contains_k_spine_if : forall σ S k e_sym e_con,
+  contains_k σ S k e_sym e_con ->
+  forall ks L_s L_c,
+    Forall3 (contains_k σ S) ks L_s L_c ->
+    forall ec et ef args,
+      unspool_app e_sym L_s = (EIf ec et ef, args) ->
+      exists kh ks' head_c args_c,
+        fold_left EApp L_c e_con = fold_left EApp args_c head_c /\
+        contains_k σ S kh (EIf ec et ef) head_c /\
+        Forall3 (contains_k σ S) ks' args args_c /\
+        kh + list_sum ks' = k + list_sum ks.
+Proof.
+  induction 1; intros kl L_s L_c HL ec0 et0 ef0 args0 Hunspool; simpl in Hunspool;
+    try discriminate Hunspool.
+  - destruct (IHcontains_k1 (ka :: kl) (a_s :: L_s) (a_c :: L_c)
+                (Forall3_cons _ _ _ _ _ _ _ H0 HL) _ _ _ _ Hunspool)
+      as [kh [ks' [hc [ac [Heq [Hh [HF Hs]]]]]]].
+    exists kh, ks', hc, ac. split; [exact Heq | split; [exact Hh | split; [exact HF | simpl in Hs; lia]]].
+  - injection Hunspool as Hc Ht Hf Hargs. subst.
+    exists (1 + smt_size ec0 + k), kl, etc, L_c.
+    split; [reflexivity | split; [apply ContK_If_True; assumption | split; [exact HL | lia]]].
+  - injection Hunspool as Hc Ht Hf Hargs. subst.
+    exists (1 + smt_size ec0 + k), kl, efc, L_c.
+    split; [reflexivity | split; [apply ContK_If_False; assumption | split; [exact HL | lia]]].
+  - exfalso.
+    apply (unspool_app_shift es [] L_s) in H. simpl in H.
+    rewrite H in Hunspool. discriminate Hunspool.
+Qed.
+
+Lemma contains_k_app_if_spine : forall σ S k e1 e2 ec et ef args e_con,
+  contains_k σ S k (EApp e1 e2) e_con ->
+  unspool_app (EApp e1 e2) [] = (EIf ec et ef, args) ->
+  exists k0, k = 1 + smt_size ec + k0 /\
+    ((models_cond σ S ec /\ contains_k σ S k0 (fold_left EApp args et) e_con) \/
+     (models_not_cond σ S ec /\ contains_k σ S k0 (fold_left EApp args ef) e_con)).
+Proof.
+  intros σ S k e1 e2 ec et ef args e_con Hc Hu.
+  destruct (contains_k_spine_if σ S k _ _ Hc nil nil nil (Forall3_nil _) ec et ef args Hu)
+    as [kh [ks' [hc [ac [Heq [Hh [HF Hs]]]]]]].
+  simpl in Heq, Hs. rewrite Heq.
+  destruct (contains_k_if_inv σ S kh ec et ef hc Hh) as [k0 [-> [[Hm Ht] | [Hm Hf]]]].
+  - exists (k0 + list_sum ks'). split; [lia |]. left. split; [exact Hm |].
+    exact (contains_k_fold_left_app σ S ks' _ _ k0 _ _ HF Ht).
+  - exists (k0 + list_sum ks'). split; [lia |]. right. split; [exact Hm |].
+    exact (contains_k_fold_left_app σ S ks' _ _ k0 _ _ HF Hf).
+Qed.
+
+End CostBasics.
+
+Section SmtCost.
+Context {sorts : SymCoreSorts} {solver : SymCoreSolver} {laws : SymFCCostLaws}.
+
+Lemma unspool_smt_size : forall e L h args,
+  unspool_app e L = (h, args) ->
+  smt_size e + list_sum (map smt_size L) + length L =
+  smt_size h + list_sum (map smt_size args) + length args.
+Proof.
+  induction e; intros L h args Hu; simpl in Hu;
+    try (injection Hu as <- <-; reflexivity).
+  apply IHe1 in Hu. simpl in *. lia.
+Qed.
+
+Lemma prim_slack_literals : forall ls,
+  prim_slack (map ELit ls) = 1 + length ls + length ls.
+Proof.
+  intros ls. unfold prim_slack. rewrite length_map.
+  assert (H : list_sum (map ground_size (map ELit ls)) = length ls).
+  { induction ls as [| l ls IH]; simpl; [reflexivity |]. rewrite IH. reflexivity. }
+  rewrite H. reflexivity.
+Qed.
+
+Lemma reduce_prim_literals_literal : forall p ls,
+  exists l0, reduce_prim p (map ELit ls) = ELit l0.
+Proof.
+  intros p ls.
+  apply reduce_prim_ground_value.
+  apply solvable_everywhere_smt_ground. intros Γ.
+  set (σ0 := fun _ : var => lit_true).
+  set (S0 := fun _ : var => false).
+  assert (Hargs : Forall2 (denote σ0 S0) (map ELit ls) ls).
+  { induction ls as [| l ls IH]; simpl; constructor; [apply denote_lit | exact IH]. }
+  destruct (reduce_prim_denote σ0 S0 p (map ELit ls) ls Hargs) as [pc [Hden _]].
+  apply (expr_to_pc_solvable Γ _ pc). apply Hden.
+  intros x Hx. discriminate Hx.
+Qed.
+
+Lemma solvable_value_contains_k : forall σ S Γ v l p args,
+  Solvable Γ v ->
+  denote σ S v l ->
+  (v = ELit l \/ (exists x, v = EVar x) \/ v = reduce_prim p args) ->
+  exists kv, kv <= smt_size v /\ contains_k σ S kv v (ELit l).
+Proof.
+  intros σ S Γ v l p args Hs Hden Hshape.
+  destruct (smt_ground v) eqn:Hg.
+  - exists 0. split; [lia |].
+    destruct Hshape as [-> | [[x ->] | Hr]]; [apply ContK_Lit | simpl in Hg; discriminate |].
+    rewrite Hr in Hg. destruct (reduce_prim_ground_value p args Hg) as [l' Hl'].
+    rewrite Hr, Hl' in *. rewrite (denote_lit_inv σ S l' l Hden). apply ContK_Lit.
+  - inversion Hs as [l' | x Hx | p0 | f a Hop Hf Ha]; subst.
+    + simpl in Hg. discriminate.
+    + destruct (denote_var_inv σ S x l Hden) as [Hsx ->].
+      exists 0. split; [lia |]. apply ContK_Var_Sym. exact Hsx.
+    + simpl in Hg. discriminate.
+    + destruct (is_op_app_unspool (EApp f a) Hop) as [p0 [args0 Hu]].
+      exists (smt_size (EApp f a)). split; [lia |].
+      destruct Hshape as [Heq | [[x Heq] | Hr]]; try discriminate Heq.
+      apply ContK_Denote with (p := p0) (args := args0); [exact Hu | | exact Hg | exact Hden].
+      rewrite Hr in Hu. exact (reduce_prim_saturated p args p0 args0 Hu).
+Qed.
+
+Lemma denote_unspool_args : forall σ S e l p args,
+  denote σ S e l -> unspool_app e [] = (EPrimOp p, args) ->
+  exists ls, Forall2 (denote σ S) args ls.
+Proof.
+  intros σ S e l p args [pc [Hden _]] Hu.
+  destruct e; simpl in Hu; try discriminate Hu.
+  - injection Hu as _ <-. exists nil. constructor.
+  - destruct (denotes_app_inv S e1 e2 pc Hden) as [p1 [pcs1 [pa [-> _]]]].
+    destruct (denotes_unspool (EApp e1 e2) S p1 (pcs1 ++ [pa]) p args Hden Hu) as [_ HF].
+    exists (map (pc_value σ) (pcs1 ++ [pa])).
+    clear Hu Hden. induction HF; simpl; constructor; [| exact IHHF].
+    exists y. split; [exact H | reflexivity].
+Qed.
+
+Definition smt_good σ S Φ Γ (e v : expr) (l : lit) : Prop :=
+  eval Inf Φ Γ e v /\ smt_size v <= 2 * smt_size e /\
+  exists kv, kv <= 2 * smt_size e /\ contains_k σ S kv v (ELit l).
+
+Lemma smt_args_eval : forall σ S Φ Γ n args args' ls,
+  (forall e v l, smt_size e < n -> denote σ S e l -> eval (Fin n) Φ Γ e v -> smt_good σ S Φ Γ e v l) ->
+  Forall (fun a => smt_size a < n) args ->
+  Forall2 (denote σ S) args ls ->
+  Forall2 (eval (Fin n) Φ Γ) args args' ->
+  Forall2 (eval Inf Φ Γ) args args' /\
+  exists ks, Forall3 (contains_k σ S) ks args' (map ELit ls) /\
+    list_sum ks <= 2 * list_sum (map smt_size args).
+Proof.
+  intros σ S Φ Γ n args args' ls IH Hsz Hden Hev. revert ls Hden Hsz.
+  induction Hev as [| a a' l1 l2 Ha _ IHl]; intros ls Hden Hsz.
+  - inversion Hden; subst. split; [constructor | exists nil; split; [constructor | simpl; lia]].
+  - inversion Hden as [| a0 l0 l1' ls' Hd Hds]; subst.
+    inversion Hsz as [| a1 l1'' Hs Hss]; subst.
+    destruct (IH a a' l0 Hs Hd Ha) as [Hinf [_ [kv [Hkv Hc]]]].
+    destruct (IHl ls' Hds Hss) as [Hinfs [ks [HF Hks]]].
+    split; [constructor; assumption |].
+    exists (kv :: ks). split; [constructor; assumption | simpl; lia].
+Qed.
+
+Lemma unspool_args_smaller : forall e p args,
+  unspool_app e [] = (EPrimOp p, args) ->
+  smt_size e = 1 + list_sum (map smt_size args) + length args.
+Proof.
+  intros e p args Hu. apply unspool_smt_size in Hu. simpl in Hu. lia.
+Qed.
+
+Lemma list_sum_map_le : forall (f : expr -> nat) l a,
+  In a l -> f a <= list_sum (map f l).
+Proof.
+  intros f l a Hin. induction l as [| b l IH]; [destruct Hin |].
+  destruct Hin as [-> | Hin]; simpl; [lia | specialize (IH Hin); lia].
+Qed.
+
+Lemma smt_eval_fin : forall σ S Φ Γ n e v l,
+  σ ⊨ Φ -> sym_free_env S Γ -> smt_size e < n -> denote σ S e l ->
+  eval (Fin n) Φ Γ e v -> smt_good σ S Φ Γ e v l.
+Proof.
+  intros σ S Φ Γ n. induction n as [| n IHn]; intros e v l Hmod Hfree Hsz Hden Hev; [lia |].
+  assert (Hsolv : Solvable Γ e).
+  { destruct Hden as [pc [Hd _]]. exact (expr_to_pc_solvable Γ e pc (Hd Γ Hfree)). }
+  inversion Hev; subst;
+    try solve [exfalso; inversion Hsolv; subst; simpl in *; congruence].
+  - match goal with [Hn : lookup_env _ _ = None |- _] =>
+      split; [apply Eval_SymVar; exact Hn | split; [simpl; lia |]] end.
+    destruct (denote_var_inv σ S x l Hden) as [Hsx ->].
+    exists 0. split; [lia | apply ContK_Var_Sym; exact Hsx].
+  - rewrite <- (denote_lit_inv σ S l0 l Hden).
+    split; [apply Eval_Lit | split; [simpl; lia | exists 0; split; [lia | apply ContK_Lit]]].
+  - exfalso.
+    match goal with [Hu : unspool_app _ _ = (ECon _, _) |- _] => apply unspool_is_con_app in Hu end.
+    rewrite (solvable_not_con_app Γ e Hsolv) in *. discriminate.
+  - exfalso. inversion Hsolv; subst.
+    match goal with [Hc : Comp _ ?f, Hs : Solvable _ ?f |- _] => exact (comp_not_solvable _ _ Hc Hs) end.
+  - match goal with
+    | [ Hu : unspool_app (EApp ef ea) [] = (EPrimOp p, ?a),
+        Hl : length ?a = primop_arity p,
+        Hargs : Forall2 _ ?a args' |- _ ] => rename a into args; rename Hu into Hun;
+                                             rename Hargs into Hev_args
+    end.
+    destruct (denote_unspool_args σ S _ l p args Hden Hun) as [ls Hls].
+    pose proof (unspool_args_smaller _ _ _ Hun) as Hse.
+    assert (Hsizes : Forall (fun a => smt_size a < n) args).
+    { apply Forall_forall. intros a Ha.
+      pose proof (list_sum_map_le smt_size args a Ha). lia. }
+    change (dec (Remaining n)) with (Fin n) in Hev_args.
+    destruct (smt_args_eval σ S Φ Γ n args args' ls
+                (fun e v l Hs Hd Hv => IHn e v l Hmod Hfree Hs Hd Hv) Hsizes Hls Hev_args)
+      as [Hinf [ks [HF Hks]]].
+    assert (Hevinf : eval Inf Φ Γ (EApp ef ea) (reduce_prim p args'))
+      by (eapply Eval_AppPrim; eassumption).
+    split; [exact Hevinf |].
+    destruct (reduce_prim_contains_k σ S p ks args' (map ELit ls) HF) as [k' [Hk' Hc']].
+    destruct (reduce_prim_literals_literal p ls) as [l0 Hl0]. rewrite Hl0 in Hc'.
+    pose proof (smt_size_contains_k _ _ _ _ _ Hc') as Hsv. simpl in Hsv.
+    rewrite prim_slack_literals in Hk'.
+    pose proof (Forall2_length Hls) as Hlen.
+    assert (Hsize : smt_size (reduce_prim p args') <= 2 * smt_size (EApp ef ea)) by lia.
+    split; [exact Hsize |].
+    pose proof (eval_denote Φ Γ σ S _ _ l Hmod Hfree Hevinf Hden) as Hden'.
+    pose proof (solvable_eval_solvable Inf Φ Γ _ _ Hevinf eq_refl (models_sat σ Φ Hmod) Hsolv) as Hsv'.
+    destruct (solvable_value_contains_k σ S Γ _ l p args' Hsv' Hden'
+                (or_intror (or_intror eq_refl))) as [kv [Hkv Hcv]].
+    exists kv. split; [lia | exact Hcv].
+  - exfalso.
+    match goal with
+    | [ Hu : unspool_app (EApp _ _) _ = (EIf _ _ _, _) |- _ ] =>
+        exact (solvable_unspool_not_if _ _ _ _ _ _ _ Hsolv Hu)
+    end.
+  - exfalso. apply models_sat in Hmod. congruence.
+Qed.
+
+End SmtCost.
+
+Ltac sym_absurd :=
+  first
+  [ match goal with [ Hs : sat _ = false, Hm : models _ _ |- _ ] =>
+      apply models_sat in Hm; congruence end
+  | match goal with [ H : unspool_app _ _ = _ |- _ ] => simpl in H; discriminate H end
+  | congruence
+  | match goal with [ Hc : Comp _ ?f, Hu : unspool_app (EApp ?f ?a) nil = _ |- _ ] =>
+      pose proof (comp_spine_head _ _ _ _ _ Hc Hu) as Hsh; simpl in *; discriminate end
+  | match goal with [ Hc : Comp _ _ |- _ ] => inversion Hc; subst; simpl in *; discriminate end ].
+
+Section Peel.
+Context {sorts : SymCoreSorts} {solver : SymCoreSolver} {laws : SymFCCostLaws}.
+Context (σ : valuation) (S : symvars).
+
+Definition good_at (A : environment -> Prop) (e_c v_c : expr) (bk be : nat) : Prop :=
+  exists h K, forall Γc Φ Γs e_s k kenv n v_s,
+    A Γc -> k <= bk -> kenv <= be -> σ ⊨ Φ ->
+    contains_env_k σ S kenv Γs Γc -> contains_k σ S k e_s e_c ->
+    h <= n -> eval (Fin n) Φ Γs e_s v_s ->
+    exists k', k' <= K /\ contains_k σ S k' v_s v_c.
+
+Definition core_at (A : environment -> Prop) (e_c v_c : expr) (bk be : nat) : Prop :=
+  exists h K, forall Γc Φ Γs e_s k kenv n v_s,
+    A Γc -> k <= bk -> kenv <= be -> σ ⊨ Φ ->
+    contains_env_k σ S kenv Γs Γc -> contains_k σ S k e_s e_c ->
+    is_if (fst (unspool_app e_s [])) = false ->
+    h <= n -> eval (Fin n) Φ Γs e_s v_s ->
+    exists k', k' <= K /\ contains_k σ S k' v_s v_c.
+
+Definition good (A : environment -> Prop) (e_c v_c : expr) : Prop :=
+  forall bk be, good_at A e_c v_c bk be.
+
+Lemma guard_true : forall Φ Γ g g' pc n,
+  σ ⊨ Φ -> sym_free_env S Γ -> models_cond σ S g -> smt_size g < n ->
+  eval (Fin n) Φ Γ g g' -> expr_to_pc Γ g' = Some pc ->
+  σ ⊨ (Φ ∧ pc) /\ smt_size g' <= 2 * smt_size g /\ models_cond σ S g'.
+Proof.
+  intros Φ Γ g g' pc n Hm Hf Hc Hs Hev Hpc.
+  destruct Hc as [pc0 [Hd Hv]].
+  destruct (smt_eval_fin σ S Φ Γ n g g' (pc_value σ pc0) Hm Hf Hs
+              (ex_intro _ pc0 (conj Hd eq_refl)) Hev) as [Hinf [Hsz _]].
+  assert (Hc' : models_cond σ S g') by
+    (eapply eval_models_cond; [exact Hm | exact Hf | exact Hinf | exists pc0; split; assumption]).
+  split; [| split; assumption].
+  apply models_and_iff. split; [exact Hm |]. exact (models_cond_pc σ S Γ g' pc Hpc Hc').
+Qed.
+
+Lemma guard_false : forall Φ Γ g g' pc n,
+  σ ⊨ Φ -> sym_free_env S Γ -> models_not_cond σ S g -> smt_size g < n ->
+  eval (Fin n) Φ Γ g g' -> expr_to_pc Γ g' = Some pc ->
+  σ ⊨ (Φ ∧ ¬ pc) /\ smt_size g' <= 2 * smt_size g /\ models_not_cond σ S g'.
+Proof.
+  intros Φ Γ g g' pc n Hm Hf Hc Hs Hev Hpc.
+  destruct Hc as [pc0 [Hd Hv]].
+  destruct (smt_eval_fin σ S Φ Γ n g g' (pc_value σ pc0) Hm Hf Hs
+              (ex_intro _ pc0 (conj Hd eq_refl)) Hev) as [Hinf [Hsz _]].
+  assert (Hc' : models_not_cond σ S g') by
+    (eapply eval_models_not_cond; [exact Hm | exact Hf | exact Hinf | exists pc0; split; assumption]).
+  split; [| split; assumption].
+  apply models_and_iff. split; [exact Hm |]. exact (models_not_cond_pc σ S Γ g' pc Hpc Hc').
+Qed.
+
+Lemma if_step_true : forall Φ Γ g t f v n,
+  σ ⊨ Φ -> sym_free_env S Γ -> models_cond σ S g -> smt_size g < n ->
+  eval (Fin (Datatypes.S n)) Φ Γ (EIf g t f) v ->
+  exists g' t' f' pc, v = EIf g' t' f' /\ eval (Fin n) (Φ ∧ pc) Γ t t' /\
+    σ ⊨ (Φ ∧ pc) /\ smt_size g' <= 2 * smt_size g /\ models_cond σ S g'.
+Proof.
+  intros Φ Γ g t f v n Hm Hf Hc Hs Hev.
+  inversion Hev; subst; try sym_absurd; change (dec (Remaining n)) with (Fin n) in *.
+  match goal with
+  | [ Hg : eval _ _ _ g ?g0, Hpc : expr_to_pc _ ?g0 = Some ?pc0 |- _ ] =>
+      destruct (guard_true Φ Γ g g0 pc0 n Hm Hf Hc Hs Hg Hpc) as [Hm' [Hsz Hc']]
+  end.
+  do 4 eexists. split; [reflexivity |]. split; [eassumption |].
+  split; [exact Hm' | split; assumption].
+Qed.
+
+Lemma if_step_false : forall Φ Γ g t f v n,
+  σ ⊨ Φ -> sym_free_env S Γ -> models_not_cond σ S g -> smt_size g < n ->
+  eval (Fin (Datatypes.S n)) Φ Γ (EIf g t f) v ->
+  exists g' t' f' pc, v = EIf g' t' f' /\ eval (Fin n) (Φ ∧ ¬ pc) Γ f f' /\
+    σ ⊨ (Φ ∧ ¬ pc) /\ smt_size g' <= 2 * smt_size g /\ models_not_cond σ S g'.
+Proof.
+  intros Φ Γ g t f v n Hm Hf Hc Hs Hev.
+  inversion Hev; subst; try sym_absurd; change (dec (Remaining n)) with (Fin n) in *.
+  match goal with
+  | [ Hg : eval _ _ _ g ?g0, Hpc : expr_to_pc _ ?g0 = Some ?pc0 |- _ ] =>
+      destruct (guard_false Φ Γ g g0 pc0 n Hm Hf Hc Hs Hg Hpc) as [Hm' [Hsz Hc']]
+  end.
+  do 4 eexists. split; [reflexivity |]. split; [eassumption |].
+  split; [exact Hm' | split; assumption].
+Qed.
+
+Lemma app_if_step : forall Φ Γ e1 e2 g t f args v n,
+  σ ⊨ Φ ->
+  unspool_app (EApp e1 e2) [] = (EIf g t f, args) ->
+  eval (Fin (Datatypes.S n)) Φ Γ (EApp e1 e2) v ->
+  eval (Fin n) Φ Γ (EIf g (fold_left EApp args t) (fold_left EApp args f)) v.
+Proof.
+  intros Φ Γ e1 e2 g t f args v n Hm Hu Hev.
+  inversion Hev; subst; try sym_absurd; change (dec (Remaining n)) with (Fin n) in *.
+  match goal with
+  | [ Hu' : unspool_app (EApp e1 e2) [] = (EIf _ _ _, _), Hr : eval _ _ _ (EIf _ _ _) v |- _ ] =>
+      rewrite Hu in Hu'; injection Hu' as <- <- <- <-; exact Hr
+  end.
+Qed.
+
+Lemma good_at_of_core : forall A e_c v_c,
+  (forall bk be, (forall bk', bk' < bk -> forall be', good_at A e_c v_c bk' be') ->
+     core_at A e_c v_c bk be) ->
+  good A e_c v_c.
+Proof.
+  intros A e_c v_c Hcore bk. induction bk as [bk IH] using lt_wf_ind. intros be.
+  destruct (Hcore bk be IH) as [hc [Kc Hc]].
+  assert (Hprev : exists h1 K1, forall Γc Φ Γs e_s k kenv n v_s,
+    A Γc -> k < bk -> kenv <= be -> σ ⊨ Φ ->
+    contains_env_k σ S kenv Γs Γc -> contains_k σ S k e_s e_c ->
+    h1 <= n -> eval (Fin n) Φ Γs e_s v_s ->
+    exists k', k' <= K1 /\ contains_k σ S k' v_s v_c).
+  { destruct bk as [| bk'].
+    - exists 0, 0. intros. lia.
+    - destruct (IH bk' ltac:(lia) be) as [h1 [K1 H1]].
+      exists h1, K1. intros Γc0 Φ0 Γs0 e0 k0 ke0 n0 v0 HA0 Hk0 Hke0 Hm0 He0 Hc0 Hn0 Hev0.
+      exact (H1 Γc0 Φ0 Γs0 e0 k0 ke0 n0 v0 HA0 ltac:(lia) Hke0 Hm0 He0 Hc0 Hn0 Hev0). }
+  destruct Hprev as [h1 [K1 H1]].
+  exists (2 + bk + hc + h1), (1 + 2 * bk + Kc + K1).
+  intros Γc Φ Γs e_s k kenv n v_s HA Hk Hkenv Hm Henv Hcont Hn Hev.
+  pose proof (contains_env_k_sym_free _ _ _ _ _ Henv) as Hfree.
+  destruct (is_if (fst (unspool_app e_s []))) eqn:Hif.
+  2: { destruct (Hc Γc Φ Γs e_s k kenv n v_s HA Hk Hkenv Hm Henv Hcont Hif ltac:(lia) Hev)
+         as [k' [Hk' Hc']].
+       exists k'. split; [lia | exact Hc']. }
+  destruct n as [| n]; [lia |].
+  destruct e_s; simpl in Hif; try discriminate Hif.
+  - change (unspool_app e_s1 [e_s2]) with (unspool_app (EApp e_s1 e_s2) []) in Hif.
+    destruct (unspool_app (EApp e_s1 e_s2) []) as [hd args] eqn:Hu.
+    simpl in Hif. destruct hd; simpl in Hif; try discriminate Hif.
+    pose proof (app_if_step Φ Γs _ _ _ _ _ _ _ n Hm Hu Hev) as Hev1.
+    destruct n as [| n]; [lia |].
+    destruct (contains_k_app_if_spine σ S k _ _ _ _ _ args e_c Hcont Hu)
+      as [k0 [Hk0 [[Hmc Harm] | [Hmc Harm]]]].
+    + destruct (if_step_true Φ Γs _ _ _ v_s n Hm Hfree Hmc ltac:(lia) Hev1)
+        as [g' [t' [f' [pc [-> [Ht [Hm' [Hsz Hc']]]]]]]].
+      destruct (H1 Γc _ Γs _ k0 kenv n t' HA ltac:(lia) Hkenv Hm' Henv Harm ltac:(lia) Ht)
+        as [k' [Hk' Hc'']].
+      exists (1 + smt_size g' + k'). split; [lia | apply ContK_If_True; assumption].
+    + destruct (if_step_false Φ Γs _ _ _ v_s n Hm Hfree Hmc ltac:(lia) Hev1)
+        as [g' [t' [f' [pc [-> [Ht [Hm' [Hsz Hc']]]]]]]].
+      destruct (H1 Γc _ Γs _ k0 kenv n f' HA ltac:(lia) Hkenv Hm' Henv Harm ltac:(lia) Ht)
+        as [k' [Hk' Hc'']].
+      exists (1 + smt_size g' + k'). split; [lia | apply ContK_If_False; assumption].
+  - destruct (contains_k_if_inv σ S k _ _ _ e_c Hcont) as [k0 [Hk0 [[Hmc Harm] | [Hmc Harm]]]].
+    + destruct (if_step_true Φ Γs _ _ _ v_s n Hm Hfree Hmc ltac:(lia) Hev)
+        as [g' [t' [f' [pc [-> [Ht [Hm' [Hsz Hc']]]]]]]].
+      destruct (H1 Γc _ Γs _ k0 kenv n t' HA ltac:(lia) Hkenv Hm' Henv Harm ltac:(lia) Ht)
+        as [k' [Hk' Hc'']].
+      exists (1 + smt_size g' + k'). split; [lia | apply ContK_If_True; assumption].
+    + destruct (if_step_false Φ Γs _ _ _ v_s n Hm Hfree Hmc ltac:(lia) Hev)
+        as [g' [t' [f' [pc [-> [Ht [Hm' [Hsz Hc']]]]]]]].
+      destruct (H1 Γc _ Γs _ k0 kenv n f' HA ltac:(lia) Hkenv Hm' Henv Harm ltac:(lia) Ht)
+        as [k' [Hk' Hc'']].
+      exists (1 + smt_size g' + k'). split; [lia | apply ContK_If_False; assumption].
+Qed.
+
+End Peel.
+
+Section NestedInduction.
+Context {sorts : SymCoreSorts} {solver : SymCoreSolver}.
+
+Variables (P : fuel -> path_condition -> environment -> expr -> expr -> Prop)
+          (Q : fuel -> path_condition -> environment -> expr -> list alt -> expr -> Prop).
+
+Hypothesis HVar : forall f Φ Γ x Γ' e e',
+  lookup_env Γ x = Some (Γ', e) -> eval (dec f) Φ Γ' e e' -> P (dec f) Φ Γ' e e' ->
+  P (Live f) Φ Γ (EVar x) e'.
+Hypothesis HSymVar : forall f Φ Γ x,
+  lookup_env Γ x = None -> P (Live f) Φ Γ (EVar x) (EVar x).
+Hypothesis HLit : forall f Φ Γ l, P (Live f) Φ Γ (ELit l) (ELit l).
+Hypothesis HCon : forall f Φ Γ e d args,
+  unspool_app e [] = (ECon d, args) ->
+  P (Live f) Φ Γ e (make_con_app d (map (delay Γ) args)).
+Hypothesis HCast : forall f Φ Γ e γ e',
+  eval (dec f) Φ Γ e e' -> P (dec f) Φ Γ e e' ->
+  P (Live f) Φ Γ (ECast e γ) (cast_expr e' γ).
+Hypothesis HAppAbs : forall f Φ Γ Γ' x eb ea eb',
+  eval (dec f) Φ (extend_env Γ' x Γ ea) eb eb' -> P (dec f) Φ (extend_env Γ' x Γ ea) eb eb' ->
+  P (Live f) Φ Γ (EApp (EThunk Γ' (ELam x eb)) ea) eb'.
+Hypothesis HAppSpine : forall f Φ Γ ef ea ef' er,
+  Comp Γ ef ->
+  eval (dec f) Φ Γ ef ef' -> P (dec f) Φ Γ ef ef' ->
+  eval (dec f) Φ Γ (EApp ef' ea) er -> P (dec f) Φ Γ (EApp ef' ea) er ->
+  P (Live f) Φ Γ (EApp ef ea) er.
+Hypothesis HBot : forall f Φ Γ b, P (Live f) Φ Γ (EBot b) (EBot b).
+Hypothesis HAppPrim : forall f Φ Γ ef ea p args args',
+  unspool_app (EApp ef ea) [] = (EPrimOp p, args) ->
+  length args = primop_arity p ->
+  Forall2 (fun a a' => eval (dec f) Φ Γ a a' /\ P (dec f) Φ Γ a a') args args' ->
+  P (Live f) Φ Γ (EApp ef ea) (reduce_prim p args').
+Hypothesis HLam : forall f Φ Γ x e, P (Live f) Φ Γ (ELam x e) (EThunk Γ (ELam x e)).
+Hypothesis HAppCast : forall f Φ Γ ef γ ea γ_a γ_r er,
+  decomp_coerc_arrow γ = Some (γ_a, γ_r) ->
+  eval (dec f) Φ Γ (ECast (EApp ef (ECast ea (sym_coerc γ_a))) γ_r) er ->
+  P (dec f) Φ Γ (ECast (EApp ef (ECast ea (sym_coerc γ_a))) γ_r) er ->
+  P (Live f) Φ Γ (EApp (ECast ef γ) ea) er.
+Hypothesis HAppIf : forall f Φ Γ e1 e2 ec et ef args er,
+  unspool_app (EApp e1 e2) [] = (EIf ec et ef, args) ->
+  eval (dec f) Φ Γ (EIf ec (fold_left EApp args et) (fold_left EApp args ef)) er ->
+  P (dec f) Φ Γ (EIf ec (fold_left EApp args et) (fold_left EApp args ef)) er ->
+  P (Live f) Φ Γ (EApp e1 e2) er.
+Hypothesis HAppBot : forall f Φ Γ b ea, P (Live f) Φ Γ (EApp (EBot b) ea) (EBot b).
+Hypothesis HCase : forall f Φ Γ es alts es' er,
+  eval (dec f) Φ Γ es es' -> P (dec f) Φ Γ es es' ->
+  fold_alts (dec f) Φ Γ (merge Γ es') alts er -> Q (dec f) Φ Γ (merge Γ es') alts er ->
+  P (Live f) Φ Γ (ECase es alts) er.
+Hypothesis HIf : forall f Φ Γ ec et ef ec' et' ef' pc_c,
+  eval (dec f) Φ Γ ec ec' -> P (dec f) Φ Γ ec ec' ->
+  expr_to_pc Γ ec' = Some pc_c ->
+  eval (dec f) (Φ ∧ pc_c) Γ et et' -> P (dec f) (Φ ∧ pc_c) Γ et et' ->
+  eval (dec f) (Φ ∧ ¬ pc_c) Γ ef ef' -> P (dec f) (Φ ∧ ¬ pc_c) Γ ef ef' ->
+  P (Live f) Φ Γ (EIf ec et ef) (EIf ec' et' ef').
+Hypothesis HCoercion : forall f Φ Γ γ, P (Live f) Φ Γ (ECoercion γ) (ECoercion (subst_coerc Γ γ)).
+Hypothesis HPrune : forall f Φ Γ e, sat Φ = false -> P (Live f) Φ Γ e (EBot BUnreachable).
+Hypothesis HType : forall f Φ Γ τ, P (Live f) Φ Γ (EType τ) (EType (subst_type Γ τ)).
+Hypothesis HThunk : forall f Φ Γ Γ' e e',
+  eval (dec f) Φ Γ' e e' -> P (dec f) Φ Γ' e e' -> P (Live f) Φ Γ (EThunk Γ' e) e'.
+Hypothesis HOutOfFuel : forall Φ Γ e, P Spent Φ Γ e (EBot BOutOfFuel).
+
+Hypothesis HFIf : forall f Φ Γ ec et ef alts et' ef' pc_c,
+  expr_to_pc Γ ec = Some pc_c ->
+  fold_alts f (Φ ∧ pc_c) Γ et alts et' -> Q f (Φ ∧ pc_c) Γ et alts et' ->
+  fold_alts f (Φ ∧ ¬ pc_c) Γ ef alts ef' -> Q f (Φ ∧ ¬ pc_c) Γ ef alts ef' ->
+  Q f Φ Γ (EIf ec et ef) alts (EIf ec et' ef').
+Hypothesis HFIfFail : forall f Φ Γ ec et ef alts,
+  expr_to_pc Γ ec = None -> Q f Φ Γ (EIf ec et ef) alts (EBot BUndefined).
+Hypothesis HFCon : forall f Φ Γ e d ea xs ep alts er,
+  decompose_con_app e = Some (d, ea) ->
+  find_alt d alts = Some (xs, ep) ->
+  eval f Φ (extend_env_multi Γ xs ea Γ) ep er -> P f Φ (extend_env_multi Γ xs ea Γ) ep er ->
+  Q f Φ Γ e alts er.
+Hypothesis HFBot : forall f Φ Γ b alts, Q f Φ Γ (EBot b) alts (EBot b).
+Hypothesis HFOtherwise : forall f Φ Γ e alts,
+  is_if (fst (unspool_app e [])) = false ->
+  (match decompose_con_app e with
+   | Some (d, _) => find_alt d alts = None
+   | None => True
+   end) ->
+  is_bot e = false ->
+  Q f Φ Γ e alts (EBot BUndefined).
+
+Fixpoint eval_nested_ind f Φ Γ e v (H : eval f Φ Γ e v) {struct H} : P f Φ Γ e v :=
+  match H in eval f Φ Γ e v return P f Φ Γ e v with
+  | Eval_Var f Φ Γ x Γ' e e' Hl He => HVar f Φ Γ x Γ' e e' Hl He (eval_nested_ind _ _ _ _ _ He)
+  | Eval_SymVar f Φ Γ x Hl => HSymVar f Φ Γ x Hl
+  | Eval_Lit f Φ Γ l => HLit f Φ Γ l
+  | Eval_Con f Φ Γ e d args Hu => HCon f Φ Γ e d args Hu
+  | Eval_Cast f Φ Γ e γ e' He => HCast f Φ Γ e γ e' He (eval_nested_ind _ _ _ _ _ He)
+  | Eval_AppAbs f Φ Γ Γ' x eb ea eb' He =>
+      HAppAbs f Φ Γ Γ' x eb ea eb' He (eval_nested_ind _ _ _ _ _ He)
+  | Eval_AppSpine f Φ Γ ef ea ef' er Hc H1 H2 =>
+      HAppSpine f Φ Γ ef ea ef' er Hc H1 (eval_nested_ind _ _ _ _ _ H1)
+        H2 (eval_nested_ind _ _ _ _ _ H2)
+  | Eval_Bot f Φ Γ b => HBot f Φ Γ b
+  | Eval_AppPrim f Φ Γ ef ea p args args' Hu Hl HF =>
+      HAppPrim f Φ Γ ef ea p args args' Hu Hl
+        ((fix go l l' (HF0 : Forall2 (eval (dec f) Φ Γ) l l') {struct HF0} :
+            Forall2 (fun a a' => eval (dec f) Φ Γ a a' /\ P (dec f) Φ Γ a a') l l' :=
+            match HF0 in Forall2 _ l l'
+              return Forall2 (fun a a' => eval (dec f) Φ Γ a a' /\ P (dec f) Φ Γ a a') l l' with
+            | @Forall2_nil _ _ _ => Forall2_nil _
+            | @Forall2_cons _ _ _ a a' l0 l0' Ha HF1 =>
+                Forall2_cons a a' (conj Ha (eval_nested_ind _ _ _ _ _ Ha)) (go l0 l0' HF1)
+            end) args args' HF)
+  | Eval_Lam f Φ Γ x e => HLam f Φ Γ x e
+  | Eval_AppCast f Φ Γ ef γ ea γ_a γ_r er Hd He =>
+      HAppCast f Φ Γ ef γ ea γ_a γ_r er Hd He (eval_nested_ind _ _ _ _ _ He)
+  | Eval_AppIf f Φ Γ e1 e2 ec et ef args er Hu He =>
+      HAppIf f Φ Γ e1 e2 ec et ef args er Hu He (eval_nested_ind _ _ _ _ _ He)
+  | Eval_AppBot f Φ Γ b ea => HAppBot f Φ Γ b ea
+  | Eval_Case f Φ Γ es alts es' er He Hf =>
+      HCase f Φ Γ es alts es' er He (eval_nested_ind _ _ _ _ _ He) Hf (fold_nested_ind _ _ _ _ _ _ Hf)
+  | Eval_If f Φ Γ ec et ef ec' et' ef' pc_c Hc Hp Ht Hf =>
+      HIf f Φ Γ ec et ef ec' et' ef' pc_c Hc (eval_nested_ind _ _ _ _ _ Hc) Hp
+        Ht (eval_nested_ind _ _ _ _ _ Ht) Hf (eval_nested_ind _ _ _ _ _ Hf)
+  | Eval_Coercion f Φ Γ γ => HCoercion f Φ Γ γ
+  | Eval_Prune f Φ Γ e Hs => HPrune f Φ Γ e Hs
+  | Eval_Type f Φ Γ τ => HType f Φ Γ τ
+  | Eval_Thunk f Φ Γ Γ' e e' He => HThunk f Φ Γ Γ' e e' He (eval_nested_ind _ _ _ _ _ He)
+  | Eval_OutOfFuel Φ Γ e => HOutOfFuel Φ Γ e
+  end
+with fold_nested_ind f Φ Γ e alts v (H : fold_alts f Φ Γ e alts v) {struct H} : Q f Φ Γ e alts v :=
+  match H in fold_alts f Φ Γ e alts v return Q f Φ Γ e alts v with
+  | FoldAlts_If f Φ Γ ec et ef alts et' ef' pc_c Hp Ht Hf =>
+      HFIf f Φ Γ ec et ef alts et' ef' pc_c Hp Ht (fold_nested_ind _ _ _ _ _ _ Ht)
+        Hf (fold_nested_ind _ _ _ _ _ _ Hf)
+  | FoldAlts_IfFail f Φ Γ ec et ef alts Hp => HFIfFail f Φ Γ ec et ef alts Hp
+  | FoldAlts_Con f Φ Γ e d ea xs ep alts er Hd Hf He =>
+      HFCon f Φ Γ e d ea xs ep alts er Hd Hf He (eval_nested_ind _ _ _ _ _ He)
+  | FoldAlts_Bot f Φ Γ b alts => HFBot f Φ Γ b alts
+  | FoldAlts_Otherwise f Φ Γ e alts H1 H2 H3 => HFOtherwise f Φ Γ e alts H1 H2 H3
+  end.
+
+End NestedInduction.
+
+Section FoldPeel.
+Context {sorts : SymCoreSorts} {solver : SymCoreSolver} {laws : SymFCCostLaws}.
+Context (σ : valuation) (S : symvars).
+
+Definition fgood_at (A : environment -> Prop) (esc : expr) (altsc : list alt) (v_c : expr)
+  (bk be : nat) : Prop :=
+  exists h K, forall Γc Φ Γs m altss k ks kenv n v_s,
+    A Γc -> k <= bk -> kenv <= be -> list_sum ks <= be -> σ ⊨ Φ ->
+    contains_env_k σ S kenv Γs Γc -> contains_k σ S k m esc ->
+    Forall3 (contains_alt_k σ S) ks altss altsc ->
+    h <= n -> fold_alts (Fin n) Φ Γs m altss v_s ->
+    exists k', k' <= K /\ contains_k σ S k' v_s v_c.
+
+Definition fcore_at (A : environment -> Prop) (esc : expr) (altsc : list alt) (v_c : expr)
+  (bk be : nat) : Prop :=
+  exists h K, forall Γc Φ Γs m altss k ks kenv n v_s,
+    A Γc -> k <= bk -> kenv <= be -> list_sum ks <= be -> σ ⊨ Φ ->
+    contains_env_k σ S kenv Γs Γc -> contains_k σ S k m esc ->
+    Forall3 (contains_alt_k σ S) ks altss altsc ->
+    is_if (fst (unspool_app m [])) = false ->
+    h <= n -> fold_alts (Fin n) Φ Γs m altss v_s ->
+    exists k', k' <= K /\ contains_k σ S k' v_s v_c.
+
+Definition fgood (A : environment -> Prop) (esc : expr) (altsc : list alt) (v_c : expr) : Prop :=
+  forall bk be, fgood_at A esc altsc v_c bk be.
+
+Lemma models_cond_expr_to_pc : forall Γ g,
+  sym_free_env S Γ -> models_cond σ S g \/ models_not_cond σ S g ->
+  exists pc, expr_to_pc Γ g = Some pc.
+Proof. intros Γ g Hf Hj. exact (models_cond_total σ S Γ g Hf Hj). Qed.
+
+Lemma fgood_of_core : forall A esc altsc v_c,
+  (forall bk be, (forall bk', bk' < bk -> forall be', fgood_at A esc altsc v_c bk' be') ->
+     fcore_at A esc altsc v_c bk be) ->
+  fgood A esc altsc v_c.
+Proof.
+  intros A esc altsc v_c Hcore bk. induction bk as [bk IH] using lt_wf_ind. intros be.
+  destruct (Hcore bk be IH) as [hc [Kc Hc]].
+  assert (Hprev : exists h1 K1, forall Γc Φ Γs m altss k ks kenv n v_s,
+    A Γc -> k < bk -> kenv <= be -> list_sum ks <= be -> σ ⊨ Φ ->
+    contains_env_k σ S kenv Γs Γc -> contains_k σ S k m esc ->
+    Forall3 (contains_alt_k σ S) ks altss altsc ->
+    h1 <= n -> fold_alts (Fin n) Φ Γs m altss v_s ->
+    exists k', k' <= K1 /\ contains_k σ S k' v_s v_c).
+  { destruct bk as [| bk'].
+    - exists 0, 0. intros. lia.
+    - destruct (IH bk' ltac:(lia) be) as [h1 [K1 H1]].
+      exists h1, K1. intros Γc0 Φ0 Γs0 m0 al0 k0 ks0 ke0 n0 v0 HA0 Hk0 Hke0 Hks0 Hm0 He0 Hc0 Ha0 Hn0 Hev0.
+      exact (H1 Γc0 Φ0 Γs0 m0 al0 k0 ks0 ke0 n0 v0 HA0 ltac:(lia) Hke0 Hks0 Hm0 He0 Hc0 Ha0 Hn0 Hev0). }
+  destruct Hprev as [h1 [K1 H1]].
+  exists (hc + h1), (1 + bk + Kc + K1).
+  intros Γc Φ Γs m altss k ks kenv n v_s HA Hk Hkenv Hks Hm Henv Hcont Halts Hn Hev.
+  pose proof (contains_env_k_sym_free _ _ _ _ _ Henv) as Hfree.
+  destruct (is_if (fst (unspool_app m []))) eqn:Hif.
+  2: { destruct (Hc Γc Φ Γs m altss k ks kenv n v_s HA Hk Hkenv Hks Hm Henv Hcont Halts Hif
+                  ltac:(lia) Hev) as [k' [Hk' Hc']].
+       exists k'. split; [lia | exact Hc']. }
+  destruct m; simpl in Hif; try discriminate Hif.
+  - exfalso.
+    change (unspool_app m1 [m2]) with (unspool_app (EApp m1 m2) []) in Hif.
+    destruct (unspool_app (EApp m1 m2) []) as [hd args] eqn:Hu.
+    simpl in Hif. destruct hd; simpl in Hif; try discriminate Hif.
+    inversion Hev; subst.
+    + match goal with [ Hd : decompose_con_app _ = Some _ |- _ ] =>
+        unfold decompose_con_app in Hd; rewrite Hu in Hd; discriminate Hd end.
+    + match goal with [ Hi : is_if (fst (unspool_app _ _)) = false |- _ ] =>
+        rewrite Hu in Hi; simpl in Hi; discriminate Hi end.
+  - destruct (contains_k_if_inv σ S k _ _ _ esc Hcont) as [k0 [Hk0 [[Hmc Harm] | [Hmc Harm]]]].
+    + inversion Hev; subst.
+      * match goal with [ Hp : expr_to_pc _ m1 = Some ?pc, Ht : fold_alts _ (Φ ∧ ?pc) _ m2 _ ?t' |- _ ] =>
+          assert (Hm' : σ ⊨ (Φ ∧ pc))
+            by (apply models_and_iff; split; [exact Hm | exact (models_cond_pc σ S Γs m1 pc Hp Hmc)]);
+          destruct (H1 Γc _ Γs m2 altss k0 ks kenv n t' HA ltac:(lia) Hkenv Hks Hm' Henv Harm Halts
+                      ltac:(lia) Ht) as [k' [Hk' Hc']];
+          exists (1 + smt_size m1 + k'); split; [lia | apply ContK_If_True; assumption]
+        end.
+      * exfalso. destruct (models_cond_expr_to_pc Γs m1 Hfree (or_introl Hmc)) as [pc Hpc]. congruence.
+      * exfalso. match goal with [ Hd : decompose_con_app _ = Some _ |- _ ] => discriminate Hd end.
+      * exfalso. match goal with [ Hi : is_if _ = false |- _ ] => discriminate Hi end.
+    + inversion Hev; subst.
+      * match goal with [ Hp : expr_to_pc _ m1 = Some ?pc, Ht : fold_alts _ (Φ ∧ ¬ ?pc) _ m3 _ ?t' |- _ ] =>
+          assert (Hm' : σ ⊨ (Φ ∧ ¬ pc))
+            by (apply models_and_iff; split; [exact Hm | exact (models_not_cond_pc σ S Γs m1 pc Hp Hmc)]);
+          destruct (H1 Γc _ Γs m3 altss k0 ks kenv n t' HA ltac:(lia) Hkenv Hks Hm' Henv Harm Halts
+                      ltac:(lia) Ht) as [k' [Hk' Hc']];
+          exists (1 + smt_size m1 + k'); split; [lia | apply ContK_If_False; assumption]
+        end.
+      * exfalso. destruct (models_cond_expr_to_pc Γs m1 Hfree (or_intror Hmc)) as [pc Hpc]. congruence.
+      * exfalso. match goal with [ Hd : decompose_con_app _ = Some _ |- _ ] => discriminate Hd end.
+      * exfalso. match goal with [ Hi : is_if _ = false |- _ ] => discriminate Hi end.
+Qed.
+
+End FoldPeel.
+
+Section Closures.
+Context {sorts : SymCoreSorts} {solver : SymCoreSolver} {laws : SymFCCostLaws}.
+Context (σ : valuation) (S : symvars).
+
+Inductive clos_tree (C : expr) : nat -> expr -> Prop :=
+  | CT_Leaf : forall k Γ x e,
+      contains_k σ S k (EThunk Γ (ELam x e)) C -> clos_tree C k (EThunk Γ (ELam x e))
+  | CT_True : forall k g t f,
+      models_cond σ S g -> clos_tree C k t -> clos_tree C (1 + smt_size g + k) (EIf g t f)
+  | CT_False : forall k g t f,
+      models_not_cond σ S g -> clos_tree C k f -> clos_tree C (1 + smt_size g + k) (EIf g t f).
+
+Lemma lam_body_value : forall Γc x ec bk be, exists h K,
+  forall Φ Γs es k kenv n v,
+    k <= bk -> kenv <= be -> σ ⊨ Φ ->
+    contains_env_k σ S kenv Γs Γc -> contains_k σ S k es (ELam x ec) ->
+    h <= n -> eval (Fin n) Φ Γs es v ->
+    exists k', k' <= K /\ clos_tree (EThunk Γc (ELam x ec)) k' v.
+Proof.
+  intros Γc x ec bk. induction bk as [bk IH] using lt_wf_ind. intros be.
+  assert (Hprev : exists h1 K1, forall Φ Γs es k kenv n v,
+    k < bk -> kenv <= be -> σ ⊨ Φ ->
+    contains_env_k σ S kenv Γs Γc -> contains_k σ S k es (ELam x ec) ->
+    h1 <= n -> eval (Fin n) Φ Γs es v ->
+    exists k', k' <= K1 /\ clos_tree (EThunk Γc (ELam x ec)) k' v).
+  { destruct bk as [| bk'].
+    - exists 0, 0. intros. lia.
+    - destruct (IH bk' ltac:(lia) be) as [h1 [K1 H1]].
+      exists h1, K1. intros Φ0 Γs0 es0 k0 ke0 n0 v0 Hk0 Hke0 Hm0 He0 Hc0 Hn0 Hev0.
+      exact (H1 Φ0 Γs0 es0 k0 ke0 n0 v0 ltac:(lia) Hke0 Hm0 He0 Hc0 Hn0 Hev0). }
+  destruct Hprev as [h1 [K1 H1]].
+  exists (2 + bk + h1), (1 + be + 2 * bk + K1).
+  intros Φ Γs es k kenv n v Hk Hkenv Hm Henv Hcont Hn Hev.
+  pose proof (contains_env_k_sym_free _ _ _ _ _ Henv) as Hfree.
+  destruct n as [| n]; [lia |].
+  inversion Hcont; subst; try (match goal with [ Ht : is_thunk _ = true |- _ ] => simpl in Ht; discriminate Ht end).
+  - inversion Hev; subst; try sym_absurd.
+    exists (kenv + k). split; [lia |].
+    apply CT_Leaf. apply ContK_Thunk; [exact Henv | apply ContK_Lam; assumption].
+  - destruct (if_step_true σ S Φ Γs _ _ _ v n Hm Hfree ltac:(eassumption) ltac:(lia) Hev)
+      as [g' [t' [f' [pc [-> [Ht [Hm' [Hsz Hc']]]]]]]].
+    destruct (H1 _ Γs _ k0 kenv n t' ltac:(lia) Hkenv Hm' Henv ltac:(eassumption) ltac:(lia) Ht)
+      as [k' [Hk' Hct]].
+    exists (1 + smt_size g' + k'). split; [lia | apply CT_True; assumption].
+  - destruct (if_step_false σ S Φ Γs _ _ _ v n Hm Hfree ltac:(eassumption) ltac:(lia) Hev)
+      as [g' [t' [f' [pc [-> [Ht [Hm' [Hsz Hc']]]]]]]].
+    destruct (H1 _ Γs _ k0 kenv n f' ltac:(lia) Hkenv Hm' Henv ltac:(eassumption) ltac:(lia) Ht)
+      as [k' [Hk' Hct]].
+    exists (1 + smt_size g' + k'). split; [lia | apply CT_False; assumption].
+Qed.
+
+Lemma clos_value : forall Γc x ec bk, exists h K,
+  forall Φ Γs es k n v,
+    k <= bk -> σ ⊨ Φ -> sym_free_env S Γs ->
+    contains_k σ S k es (EThunk Γc (ELam x ec)) ->
+    h <= n -> eval (Fin n) Φ Γs es v ->
+    exists k', k' <= K /\ clos_tree (EThunk Γc (ELam x ec)) k' v.
+Proof.
+  intros Γc x ec bk. induction bk as [bk IH] using lt_wf_ind.
+  assert (Hprev : exists h1 K1, forall Φ Γs es k n v,
+    k < bk -> σ ⊨ Φ -> sym_free_env S Γs ->
+    contains_k σ S k es (EThunk Γc (ELam x ec)) ->
+    h1 <= n -> eval (Fin n) Φ Γs es v ->
+    exists k', k' <= K1 /\ clos_tree (EThunk Γc (ELam x ec)) k' v).
+  { destruct bk as [| bk'].
+    - exists 0, 0. intros. lia.
+    - destruct (IH bk' ltac:(lia)) as [h1 [K1 H1]].
+      exists h1, K1. intros Φ0 Γs0 es0 k0 n0 v0 Hk0 Hm0 Hf0 Hc0 Hn0 Hev0.
+      exact (H1 Φ0 Γs0 es0 k0 n0 v0 ltac:(lia) Hm0 Hf0 Hc0 Hn0 Hev0). }
+  destruct Hprev as [h1 [K1 H1]].
+  destruct (lam_body_value Γc x ec bk bk) as [hl [Kl Hl]].
+  exists (2 + bk + h1 + hl), (1 + 2 * bk + K1 + Kl).
+  intros Φ Γs es k n v Hk Hm Hfree Hcont Hn Hev.
+  destruct n as [| n]; [lia |].
+  inversion Hcont; subst.
+  - inversion Hev; subst; try sym_absurd.
+    change (dec (Remaining n)) with (Fin n) in *.
+    match goal with
+    | [ He : contains_env_k _ _ ?ke ?G _, Hb : contains_k _ _ ?kb ?b (ELam _ _),
+        Hv : eval (Fin n) _ ?G ?b v |- _ ] =>
+        destruct (Hl Φ G b kb ke n v ltac:(lia) ltac:(lia) Hm He Hb ltac:(lia) Hv) as [k' [Hk' Hct]]
+    end.
+    exists k'. split; [lia | exact Hct].
+  - inversion Hev; subst; try sym_absurd.
+    change (dec (Remaining n)) with (Fin n) in *.
+    match goal with
+    | [ He : contains_env_k _ _ ?ke ?G _, Hb : contains_k _ _ ?kb ?b (EThunk _ _),
+        Hv : eval (Fin n) _ ?G ?b v |- _ ] =>
+        destruct (H1 Φ G b kb n v ltac:(lia) Hm (contains_env_k_sym_free _ _ _ _ _ He) Hb ltac:(lia) Hv)
+          as [k' [Hk' Hct]]
+    end.
+    exists k'. split; [lia | exact Hct].
+  - destruct (if_step_true σ S Φ Γs _ _ _ v n Hm Hfree ltac:(eassumption) ltac:(lia) Hev)
+      as [g' [t' [f' [pc [-> [Ht [Hm' [Hsz Hc']]]]]]]].
+    destruct (H1 _ Γs _ k0 n t' ltac:(lia) Hm' Hfree ltac:(eassumption) ltac:(lia) Ht)
+      as [k' [Hk' Hct]].
+    exists (1 + smt_size g' + k'). split; [lia | apply CT_True; assumption].
+  - destruct (if_step_false σ S Φ Γs _ _ _ v n Hm Hfree ltac:(eassumption) ltac:(lia) Hev)
+      as [g' [t' [f' [pc [-> [Ht [Hm' [Hsz Hc']]]]]]]].
+    destruct (H1 _ Γs _ k0 n f' ltac:(lia) Hm' Hfree ltac:(eassumption) ltac:(lia) Ht)
+      as [k' [Hk' Hct]].
+    exists (1 + smt_size g' + k'). split; [lia | apply CT_False; assumption].
+Qed.
+
+Lemma clos_tree_contains : forall C k m, clos_tree C k m -> contains_k σ S k m C.
+Proof.
+  intros C k m H. induction H.
+  - assumption.
+  - apply ContK_If_True; assumption.
+  - apply ContK_If_False; assumption.
+Qed.
+
+Section AppAbs.
+Variables (Γc0 Γc' : environment) (x : var) (eb ea v_c : expr).
+Hypothesis Hbody : good σ S (eq (extend_env Γc' x Γc0 ea)) eb v_c.
+Hypothesis Hea : concore_expr ea.
+
+Lemma app_abs_tree : forall bk be, exists h K,
+  forall Φ Γs f a kf ka kenv n v_s,
+    kf <= bk -> ka <= be -> kenv <= be -> σ ⊨ Φ ->
+    contains_env_k σ S kenv Γs Γc0 ->
+    clos_tree (EThunk Γc' (ELam x eb)) kf f -> contains_k σ S ka a ea ->
+    h <= n -> eval (Fin n) Φ Γs (EApp f a) v_s ->
+    exists k', k' <= K /\ contains_k σ S k' v_s v_c.
+Proof.
+  intros bk. induction bk as [bk IH] using lt_wf_ind. intros be.
+  assert (Hprev : exists h1 K1, forall Φ Γs f a kf ka kenv n v_s,
+    kf < bk -> ka <= be -> kenv <= be -> σ ⊨ Φ ->
+    contains_env_k σ S kenv Γs Γc0 ->
+    clos_tree (EThunk Γc' (ELam x eb)) kf f -> contains_k σ S ka a ea ->
+    h1 <= n -> eval (Fin n) Φ Γs (EApp f a) v_s ->
+    exists k', k' <= K1 /\ contains_k σ S k' v_s v_c).
+  { destruct bk as [| bk'].
+    - exists 0, 0. intros. lia.
+    - destruct (IH bk' ltac:(lia) be) as [h1 [K1 H1]].
+      exists h1, K1. intros Φ0 Γs0 f0 a0 kf0 ka0 ke0 n0 v0 Hkf0 Hka0 Hke0 Hm0 He0 Ht0 Ha0 Hn0 Hev0.
+      exact (H1 Φ0 Γs0 f0 a0 kf0 ka0 ke0 n0 v0 ltac:(lia) Hka0 Hke0 Hm0 He0 Ht0 Ha0 Hn0 Hev0). }
+  destruct Hprev as [h1 [K1 H1]].
+  destruct (Hbody bk (be + be + bk)) as [h0 [K0 H0]].
+  exists (2 + bk + h0 + h1), (1 + 2 * bk + K0 + K1).
+  intros Φ Γs f a kf ka kenv n v_s Hkf Hka Hkenv Hm Henv Htree Ha Hn Hev.
+  pose proof (contains_env_k_sym_free _ _ _ _ _ Henv) as Hfree.
+  destruct n as [| n]; [lia |].
+  inversion Htree; subst.
+  - match goal with [ Hc : contains_k _ _ _ (EThunk _ (ELam _ _)) _ |- _ ] =>
+      destruct (contains_k_clos_inv σ S _ _ _ _ _ Hc)
+        as [Γc2 [bodyc [kenv1 [kb [Heq [Hsx [Henv1 [Hb Hkk]]]]]]]] end.
+    injection Heq as <- <- <-.
+    inversion Hev; subst; try sym_absurd.
+    change (dec (Remaining n)) with (Fin n) in *.
+    match goal with [ Hv : eval (Fin n) Φ (extend_env _ _ _ _) _ v_s |- _ ] => rename Hv into Hbody_ev end.
+    assert (Hext : contains_env_k σ S (kenv + ka + kenv1)
+                     (extend_env Γ x Γs a) (extend_env Γc' x Γc0 ea)).
+    { unfold extend_env. apply ContK_Env_Extend; assumption. }
+    destruct (H0 _ Φ _ _ kb (kenv + ka + kenv1) n v_s eq_refl ltac:(lia) ltac:(lia) Hm Hext Hb
+                ltac:(lia) Hbody_ev) as [k' [Hk' Hc']].
+    exists k'. split; [lia | exact Hc'].
+  - assert (Hu : unspool_app (EApp (EIf g t f0) a) [] = (EIf g t f0, [a])) by reflexivity.
+    pose proof (app_if_step σ Φ Γs _ _ _ _ _ _ _ n Hm Hu Hev) as Hev1. simpl in Hev1.
+    destruct n as [| n]; [lia |].
+    destruct (if_step_true σ S Φ Γs _ _ _ v_s n Hm Hfree ltac:(eassumption) ltac:(lia) Hev1)
+      as [g' [t' [f' [pc [-> [Ht [Hm' [Hsz Hc']]]]]]]].
+    destruct (H1 _ Γs t a k ka kenv n t' ltac:(lia) Hka Hkenv Hm' Henv ltac:(eassumption) Ha
+                ltac:(lia) Ht) as [k' [Hk' Hct]].
+    exists (1 + smt_size g' + k'). split; [lia | apply ContK_If_True; assumption].
+  - assert (Hu : unspool_app (EApp (EIf g t f0) a) [] = (EIf g t f0, [a])) by reflexivity.
+    pose proof (app_if_step σ Φ Γs _ _ _ _ _ _ _ n Hm Hu Hev) as Hev1. simpl in Hev1.
+    destruct n as [| n]; [lia |].
+    destruct (if_step_false σ S Φ Γs _ _ _ v_s n Hm Hfree ltac:(eassumption) ltac:(lia) Hev1)
+      as [g' [t' [f' [pc [-> [Ht [Hm' [Hsz Hc']]]]]]]].
+    destruct (H1 _ Γs f0 a k ka kenv n f' ltac:(lia) Hka Hkenv Hm' Henv ltac:(eassumption) Ha
+                ltac:(lia) Ht) as [k' [Hk' Hct]].
+    exists (1 + smt_size g' + k'). split; [lia | apply ContK_If_False; assumption].
+Qed.
+
+Lemma app_abs_core : forall bk be,
+  core_at σ S (eq Γc0) (EApp (EThunk Γc' (ELam x eb)) ea) v_c bk be.
+Proof.
+  intros bk be.
+  destruct (clos_value Γc' x eb bk) as [hc [Kc Hc]].
+  destruct (app_abs_tree (bk + Kc) (be + bk)) as [hL [KL HL]].
+  exists (1 + hc + hL), KL.
+  intros Γc Φ Γs e_s k kenv n v_s HA Hk Hkenv Hm Henv Hcont Hif Hn Hev. subst Γc.
+  pose proof (contains_env_k_sym_free _ _ _ _ _ Henv) as Hfree.
+  destruct n as [| n]; [lia |].
+  inversion Hcont; subst; try (simpl in Hif; discriminate Hif);
+    try (match goal with [ Ht : is_thunk _ = true |- _ ] => simpl in Ht; discriminate Ht end).
+  match goal with [ Hf : contains_k _ _ ?kf ?f (EThunk _ _), Ha : contains_k _ _ ?ka ?a ea |- _ ] =>
+    rename Hf into Hfc; rename Ha into Hac; rename f into fs; rename a into as_;
+    rename kf into kfs; rename ka into kas end.
+  destruct fs; try (inversion Hfc; fail); try (simpl in Hif; discriminate Hif).
+  inversion Hev; subst; try sym_absurd.
+  - exact (HL Φ Γs _ as_ kfs kas kenv (Datatypes.S n) v_s ltac:(lia) ltac:(lia) ltac:(lia) Hm Henv
+             (CT_Leaf _ _ _ _ _ Hfc) Hac ltac:(lia) Hev).
+  - change (dec (Remaining n)) with (Fin n) in *.
+    match goal with
+    | [ H1 : eval (Fin n) Φ Γs (EThunk _ _) ?f', H2 : eval (Fin n) Φ Γs (EApp ?f' as_) v_s |- _ ] =>
+        destruct (Hc Φ Γs _ kfs n f' ltac:(lia) Hm Hfree Hfc ltac:(lia) H1) as [k' [Hk' Ht']];
+        exact (HL Φ Γs f' as_ k' kas kenv n v_s ltac:(lia) ltac:(lia) ltac:(lia) Hm Henv Ht' Hac
+                 ltac:(lia) H2)
+    end.
+Qed.
+
+End AppAbs.
+
+End Closures.
+
+Ltac cont_absurd Hif :=
+  first
+  [ simpl in Hif; discriminate Hif
+  | match goal with [ Ht : is_thunk _ = true |- _ ] => simpl in Ht; discriminate Ht end
+  | match goal with [ Hu : unspool_app _ _ = _ |- _ ] => simpl in Hu; discriminate Hu end ].
+
+Section SimpleCores.
+Context {sorts : SymCoreSorts} {solver : SymCoreSolver} {laws : SymFCCostLaws}.
+Context (σ : valuation) (S : symvars).
+
+Lemma var_core : forall Γc0 x Γc' e0 v bk be,
+  lookup_env Γc0 x = Some (Γc', e0) ->
+  good σ S (eq Γc') e0 v ->
+  core_at σ S (eq Γc0) (EVar x) v bk be.
+Proof.
+  intros Γc0 x Γc' e0 v bk be Hl IH.
+  destruct (IH be be) as [h0 [K0 H0]].
+  exists (1 + h0), K0.
+  intros Γc Φ Γs e_s k kenv n v_s HA Hk Hkenv Hm Henv Hcont Hif Hn Hev. subst Γc.
+  destruct n as [| n]; [lia |].
+  inversion Hcont; subst; try cont_absurd Hif.
+  inversion Hev; subst; try sym_absurd.
+  - change (dec (Remaining n)) with (Fin n) in *.
+    match goal with [ Hls : lookup_env Γs x = Some (?G, ?b), Hb : eval (Fin n) Φ ?G ?b v_s |- _ ] =>
+      destruct (contains_env_k_lookup σ S kenv Γs Γc0 x G b Henv Hls)
+        as [Gc [ec [k1 [k2 [Hlc [Hce1 [Hce2 [Hk1 Hk2]]]]]]]];
+      rewrite Hl in Hlc; injection Hlc as HG He; subst Gc ec;
+      exact (H0 Γc' Φ G b k2 k1 n v_s eq_refl ltac:(lia) ltac:(lia) Hm Hce1 Hce2 ltac:(lia) Hb)
+    end.
+  - exfalso.
+    match goal with [ Hls : lookup_env Γs x = None |- _ ] =>
+      pose proof (contains_env_lookup_none σ S Γs Γc0 x (contains_env_k_erase _ _ _ _ _ Henv) Hls) as Hc
+    end.
+    congruence.
+Qed.
+
+Lemma symvar_core : forall Γc0 x bk be,
+  lookup_env Γc0 x = None ->
+  core_at σ S (eq Γc0) (EVar x) (EVar x) bk be.
+Proof.
+  intros Γc0 x bk be Hl.
+  exists 1, 0.
+  intros Γc Φ Γs e_s k kenv n v_s HA Hk Hkenv Hm Henv Hcont Hif Hn Hev. subst Γc.
+  destruct n as [| n]; [lia |].
+  inversion Hcont; subst; try cont_absurd Hif.
+  inversion Hev; subst; try sym_absurd.
+  - exfalso.
+    match goal with [ Hls : lookup_env Γs x = Some (?G, ?b) |- _ ] =>
+      destruct (contains_env_k_lookup σ S kenv Γs Γc0 x G b Henv Hls)
+        as [Gc [ec [k1 [k2 [Hlc _]]]]]
+    end.
+    congruence.
+  - exists 0. split; [lia | apply ContK_Var_Bound; assumption].
+Qed.
+
+Lemma lit_core : forall Γc0 l bk be,
+  core_at σ S (eq Γc0) (ELit l) (ELit l) bk be.
+Proof.
+  intros Γc0 l bk be.
+  exists (1 + bk), (2 * bk).
+  intros Γc Φ Γs e_s k kenv n v_s HA Hk Hkenv Hm Henv Hcont Hif Hn Hev. subst Γc.
+  pose proof (contains_env_k_sym_free _ _ _ _ _ Henv) as Hfree.
+  inversion Hcont; subst; try cont_absurd Hif.
+  - destruct n as [| n]; [lia |].
+    inversion Hev; subst; try sym_absurd.
+    + exfalso.
+      match goal with [ Hls : lookup_env Γs ?y = Some _, Hsy : S ?y = true |- _ ] =>
+        rewrite (Hfree y Hsy) in Hls; discriminate Hls end.
+    + exists 0. split; [lia | apply ContK_Var_Sym; assumption].
+  - destruct n as [| n]; [lia |].
+    inversion Hev; subst; try sym_absurd.
+    exists 0. split; [lia | apply ContK_Lit].
+  - match goal with [ Hd : denote σ S e_s l |- _ ] =>
+      destruct (smt_eval_fin σ S Φ Γs n e_s v_s l Hm Hfree ltac:(lia) Hd Hev)
+        as [_ [_ [kv [Hkv Hc]]]]
+    end.
+    exists kv. split; [lia | exact Hc].
+Qed.
+
+Lemma lam_core : forall Γc0 x e bk be,
+  core_at σ S (eq Γc0) (ELam x e) (EThunk Γc0 (ELam x e)) bk be.
+Proof.
+  intros Γc0 x e bk be.
+  exists 1, (be + bk).
+  intros Γc Φ Γs e_s k kenv n v_s HA Hk Hkenv Hm Henv Hcont Hif Hn Hev. subst Γc.
+  destruct n as [| n]; [lia |].
+  inversion Hcont; subst; try cont_absurd Hif.
+  inversion Hev; subst; try sym_absurd.
+  exists (kenv + k). split; [lia |].
+  apply ContK_Thunk; [exact Henv | apply ContK_Lam; assumption].
+Qed.
+
+Lemma bot_core : forall Γc0 b bk be,
+  core_at σ S (eq Γc0) (EBot b) (EBot b) bk be.
+Proof.
+  intros Γc0 b bk be.
+  exists 1, 0.
+  intros Γc Φ Γs e_s k kenv n v_s HA Hk Hkenv Hm Henv Hcont Hif Hn Hev. subst Γc.
+  destruct n as [| n]; [lia |].
+  inversion Hcont; subst; try cont_absurd Hif.
+  inversion Hev; subst; try sym_absurd.
+  exists 0. split; [lia | apply ContK_Bot].
+Qed.
+
+Lemma contains_coercion_eq : forall a b, contains σ S (ECoercion a) (ECoercion b) -> a = b.
+Proof. intros a b H. inversion H; subst; try reflexivity; simpl in *; discriminate. Qed.
+
+Lemma contains_type_eq : forall a b, contains σ S (EType a) (EType b) -> a = b.
+Proof. intros a b H. inversion H; subst; try reflexivity; simpl in *; discriminate. Qed.
+
+Lemma coercion_core : forall Γc0 γ bk be,
+  core_at σ S (eq Γc0) (ECoercion γ) (ECoercion (subst_coerc Γc0 γ)) bk be.
+Proof.
+  intros Γc0 γ bk be.
+  exists 1, 0.
+  intros Γc Φ Γs e_s k kenv n v_s HA Hk Hkenv Hm Henv Hcont Hif Hn Hev. subst Γc.
+  destruct n as [| n]; [lia |].
+  inversion Hcont; subst; try cont_absurd Hif.
+  inversion Hev; subst; try sym_absurd.
+  rewrite (contains_coercion_eq _ _
+             (subst_coerc_contains_env σ S Γs Γc0 γ (contains_env_k_erase _ _ _ _ _ Henv))).
+  exists 0. split; [lia | apply ContK_Coercion].
+Qed.
+
+Lemma type_core : forall Γc0 τ bk be,
+  core_at σ S (eq Γc0) (EType τ) (EType (subst_type Γc0 τ)) bk be.
+Proof.
+  intros Γc0 τ bk be.
+  exists 1, 0.
+  intros Γc Φ Γs e_s k kenv n v_s HA Hk Hkenv Hm Henv Hcont Hif Hn Hev. subst Γc.
+  destruct n as [| n]; [lia |].
+  inversion Hcont; subst; try cont_absurd Hif.
+  inversion Hev; subst; try sym_absurd.
+  rewrite (contains_type_eq _ _
+             (subst_type_contains_env σ S Γs Γc0 τ (contains_env_k_erase _ _ _ _ _ Henv))).
+  exists 0. split; [lia | apply ContK_Type].
+Qed.
+
+Lemma app_bot_core : forall Γc0 b c2 bk be,
+  core_at σ S (eq Γc0) (EApp (EBot b) c2) (EBot b) bk be.
+Proof.
+  intros Γc0 b c2 bk be.
+  exists 1, 0.
+  intros Γc Φ Γs e_s k kenv n v_s HA Hk Hkenv Hm Henv Hcont Hif Hn Hev. subst Γc.
+  destruct n as [| n]; [lia |].
+  inversion Hcont; subst; try cont_absurd Hif.
+  match goal with [ Hf : contains_k _ _ _ ?f (EBot b) |- _ ] =>
+    inversion Hf; subst; try cont_absurd Hif end.
+  inversion Hev; subst; try sym_absurd.
+  exists 0. split; [lia | apply ContK_Bot].
+Qed.
+
+Lemma cast_core : forall Γc0 c γ c' bk be,
+  good σ S (eq Γc0) c c' ->
+  core_at σ S (eq Γc0) (ECast c γ) (cast_expr c' γ) bk be.
+Proof.
+  intros Γc0 c γ c' bk be IH.
+  destruct (IH bk be) as [h0 [K0 H0]].
+  exists (1 + h0), K0.
+  intros Γc Φ Γs e_s k kenv n v_s HA Hk Hkenv Hm Henv Hcont Hif Hn Hev. subst Γc.
+  destruct n as [| n]; [lia |].
+  inversion Hcont; subst; try cont_absurd Hif.
+  inversion Hev; subst; try sym_absurd.
+  change (dec (Remaining n)) with (Fin n) in *.
+  match goal with [ Hc : contains_k _ _ k ?es c, Hv : eval (Fin n) Φ Γs ?es ?es' |- _ ] =>
+    destruct (H0 Γc0 Φ Γs es k kenv n es' eq_refl Hk Hkenv Hm Henv Hc ltac:(lia) Hv)
+      as [k' [Hk' Hc']];
+    exists k'; split; [exact Hk' | apply cast_expr_contains_k; exact Hc']
+  end.
+Qed.
+
+Lemma app_cast_core : forall Γc0 c γ c2 γ_a γ_r v bk be,
+  decomp_coerc_arrow γ = Some (γ_a, γ_r) ->
+  good σ S (eq Γc0) (ECast (EApp c (ECast c2 (sym_coerc γ_a))) γ_r) v ->
+  core_at σ S (eq Γc0) (EApp (ECast c γ) c2) v bk be.
+Proof.
+  intros Γc0 c γ c2 γ_a γ_r v bk be Hd IH.
+  destruct (IH bk be) as [h0 [K0 H0]].
+  exists (1 + h0), K0.
+  intros Γc Φ Γs e_s k kenv n v_s HA Hk Hkenv Hm Henv Hcont Hif Hn Hev. subst Γc.
+  destruct n as [| n]; [lia |].
+  inversion Hcont; subst; try cont_absurd Hif.
+  match goal with [ Hf : contains_k _ _ _ ?f (ECast c γ) |- _ ] =>
+    inversion Hf; subst; try cont_absurd Hif end.
+  inversion Hev; subst; try sym_absurd.
+  change (dec (Remaining n)) with (Fin n) in *.
+  match goal with
+  | [ Hd' : decomp_coerc_arrow γ = Some _, Hv : eval (Fin n) Φ Γs _ v_s,
+      Hfs : contains_k _ _ ?kf ?fs c, Has : contains_k _ _ ?ka ?as0 c2 |- _ ] =>
+      rewrite Hd in Hd'; injection Hd' as <- <-;
+      exact (H0 Γc0 Φ Γs _ (kf + ka) kenv n v_s eq_refl Hk Hkenv Hm Henv
+               (ContK_Cast _ _ _ _ _ γ_r (ContK_App _ _ _ _ _ _ _ _ Hfs (ContK_Cast _ _ _ _ _ _ Has)))
+               ltac:(lia) Hv)
+  end.
+Qed.
+
+End SimpleCores.
+
+Section SpineCores.
+Context {sorts : SymCoreSorts} {solver : SymCoreSolver} {laws : SymFCCostLaws}.
+Context (σ : valuation) (S : symvars).
+
+Definition rigid_head (h : expr) : bool :=
+  match h with
+  | ECon _ | EPrimOp _ => true
+  | _ => false
+  end.
+
+Lemma contains_k_unspool_rigid_rev : forall k e_s e_c,
+  contains_k σ S k e_s e_c ->
+  forall kl Ls Lc h args_c,
+    Forall3 (contains_k σ S) kl Ls Lc ->
+    unspool_app e_c Lc = (h, args_c) ->
+    rigid_head h = true ->
+    is_if (fst (unspool_app e_s Ls)) = false ->
+    exists args_s ks,
+      unspool_app e_s Ls = (h, args_s) /\ Forall3 (contains_k σ S) ks args_s args_c /\
+      list_sum ks = k + list_sum kl.
+Proof.
+  induction 1; intros kl Ls Lc h args_c HL Hu Hr Hif; simpl in Hu, Hif |- *;
+    try (injection Hu as <- <-; simpl in Hr; discriminate Hr).
+  - injection Hu as <- <-. exists Ls, kl. split; [reflexivity | split; [exact HL | reflexivity]].
+  - injection Hu as <- <-. exists Ls, kl. split; [reflexivity | split; [exact HL | reflexivity]].
+  - destruct (IHcontains_k1 (ka :: kl) (a_s :: Ls) (a_c :: Lc) h args_c
+                (Forall3_cons _ _ _ _ _ _ _ H0 HL) Hu Hr Hif) as [args_s [ks [Hus [HF Hs]]]].
+    exists args_s, ks. split; [exact Hus | split; [exact HF | simpl in Hs; lia]].
+  - destruct ec; simpl in H1; try discriminate H1.
+    simpl in Hu. injection Hu as <- <-. simpl in Hr. discriminate Hr.
+  - discriminate Hif.
+  - discriminate Hif.
+Qed.
+
+Lemma find_alt_contains_alt_k_rev : forall ks altss altsc d xs epc,
+  Forall3 (contains_alt_k σ S) ks altss altsc ->
+  find_alt d altsc = Some (xs, epc) ->
+  exists eps kp, find_alt d altss = Some (xs, eps) /\ Forall (fun x => S x = false) xs /\
+    contains_k σ S kp eps epc /\ kp <= list_sum ks.
+Proof.
+  intros ks altss altsc d xs epc HF. revert xs epc.
+  induction HF as [| k a_s a_c ks la lc Ha _ IH]; intros xs epc Hf; simpl in Hf; [discriminate |].
+  inversion Ha as [k0 d0 xs0 eps epc0 Hxs Hb]; subst. simpl.
+  destruct (string_dec d d0).
+  - injection Hf as <- <-. exists eps, k. repeat split; try assumption. simpl. lia.
+  - destruct (IH xs epc Hf) as [eps' [kp [H1 [H2 [H3 H4]]]]].
+    exists eps', kp. repeat split; try assumption. simpl. lia.
+Qed.
+
+Lemma extend_env_multi_contains_k : forall xs kΓ ka ks Γs Γc Γas Γac args_s args_c,
+  Forall (fun x => S x = false) xs ->
+  contains_env_k σ S kΓ Γs Γc ->
+  contains_env_k σ S ka Γas Γac ->
+  Forall3 (contains_k σ S) ks args_s args_c ->
+  Forall concore_expr args_c ->
+  exists k', k' <= kΓ + length xs * (ka + list_sum ks) /\
+    contains_env_k σ S k' (extend_env_multi Γs xs args_s Γas) (extend_env_multi Γc xs args_c Γac).
+Proof.
+  induction xs as [| x xs IH]; intros kΓ ka ks Γs Γc Γas Γac args_s args_c Hxs HΓ Ha HF Hcon.
+  - exists kΓ. split; [lia | exact HΓ].
+  - inversion Hxs as [| x0 xs0 Hx Hxs']; subst.
+    destruct HF as [| k a_s a_c ks' l1 l2 Hac HF'].
+    + destruct (IH kΓ ka nil Γs Γc Γas Γac nil nil Hxs' HΓ Ha (Forall3_nil _) Hcon) as [k' [Hk' Hc']].
+      exists (ka + 0 + k'). split; [simpl in *; nia |].
+      simpl. unfold extend_env. apply ContK_Env_Extend;
+        [exact Hx | exact Ha | apply ContK_Bot | constructor | exact Hc'].
+    + inversion Hcon as [| c0 cs Hc0 Hcs]; subst.
+      destruct (IH kΓ ka ks' Γs Γc Γas Γac l1 l2 Hxs' HΓ Ha HF' Hcs) as [k' [Hk' Hc']].
+      exists (ka + k + k'). split; [simpl in *; nia |].
+      simpl. unfold extend_env. apply ContK_Env_Extend; assumption.
+Qed.
+
+Lemma spine_head_rev : forall k f c,
+  contains_k σ S k f c ->
+  is_if (spine_head f) = false ->
+  has_whole_spine_rule (spine_head c) = false ->
+  (forall l, spine_head c <> ELit l) ->
+  has_whole_spine_rule (spine_head f) = false.
+Proof.
+  induction 1; intros Hif Hw Hl; simpl in *; try reflexivity; try discriminate.
+  - exact (IHcontains_k1 Hif Hw Hl).
+  - exfalso. exact (Hl l eq_refl).
+Qed.
+
+Lemma comp_k_rev : forall kenv k Γs Γc f c,
+  contains_env_k σ S kenv Γs Γc ->
+  contains_k σ S k f c ->
+  Comp Γc c ->
+  is_if (spine_head f) = false ->
+  (forall l, spine_head c <> ELit l) ->
+  Comp Γs f.
+Proof.
+  intros kenv k Γs Γc f c Henv Hc Hcomp Hif Hl.
+  destruct Hcomp as [x Hbound | x body | es alts | Γ' e Hnotlam | ef ea Hhead].
+  - inversion Hc; subst; simpl in Hif; try discriminate Hif;
+      try (match goal with [ Ht : is_thunk _ = true |- _ ] => simpl in Ht; discriminate Ht end).
+    apply Comp_Var. intros Hnone. apply Hbound.
+    exact (contains_env_lookup_none σ S Γs Γc x (contains_env_k_erase _ _ _ _ _ Henv) Hnone).
+  - inversion Hc; subst; simpl in Hif; try discriminate Hif;
+      try (match goal with [ Ht : is_thunk _ = true |- _ ] => simpl in Ht; discriminate Ht end). apply Comp_Lam.
+  - inversion Hc; subst; simpl in Hif; try discriminate Hif;
+      try (match goal with [ Ht : is_thunk _ = true |- _ ] => simpl in Ht; discriminate Ht end). apply Comp_Case.
+  - inversion Hc; subst; simpl in Hif; try discriminate Hif;
+      try (match goal with [ Ht : is_thunk _ = true |- _ ] => simpl in Ht; discriminate Ht end).
+    + apply Comp_Thunk.
+      match goal with [ Hb : contains_k _ _ _ ?b e |- is_lam ?b = false ] =>
+        destruct b; try reflexivity; inversion Hb; subst; simpl in Hnotlam; discriminate end.
+    + apply Comp_Thunk.
+      match goal with [ Hb : contains_k _ _ _ ?b (EThunk Γ' e) |- is_lam ?b = false ] =>
+        destruct b; try reflexivity; inversion Hb end.
+  - inversion Hc; subst; simpl in Hif; try discriminate Hif;
+      try (match goal with [ Ht : is_thunk _ = true |- _ ] => simpl in Ht; discriminate Ht end).
+    apply Comp_App. exact (spine_head_rev _ _ _ Hc Hif Hhead Hl).
+Qed.
+
+Lemma eval_spine_head_lit : forall f Φ Γ e v,
+  eval f Φ Γ e v -> f = Inf -> Φ = pc_true ->
+  forall l, spine_head e = ELit l -> e = ELit l.
+Proof.
+  intros f Φ Γ e v H. induction H; intros Hf HΦ l0 Hl; try discriminate Hf; subst;
+    simpl in Hl; try exact Hl; try discriminate Hl;
+    try (rewrite sat_pc_true in *; discriminate).
+  - rewrite <- (fst_unspool_app e []) in Hl.
+    match goal with [ Hu : unspool_app e [] = _ |- _ ] => rewrite Hu in Hl end.
+    discriminate Hl.
+  - injection Hf as Hf. subst f.
+    specialize (IHeval1 eq_refl eq_refl l0 Hl). subst ef. inversion H.
+  - pose proof (fst_unspool_app (EApp ef ea) []) as Hs.
+    match goal with [ Hu : unspool_app (EApp ef ea) [] = _ |- _ ] => rewrite Hu in Hs end.
+    simpl in Hs. rewrite Hl in Hs. discriminate Hs.
+  - pose proof (fst_unspool_app (EApp e1 e2) []) as Hs.
+    match goal with [ Hu : unspool_app (EApp e1 e2) [] = _ |- _ ] => rewrite Hu in Hs end.
+    simpl in Hs. rewrite Hl in Hs. discriminate Hs.
+Qed.
+
+End SpineCores.
+
+Section MoreCores.
+Context {sorts : SymCoreSorts} {solver : SymCoreSolver} {laws : SymFCCostLaws}.
+Context (σ : valuation) (S : symvars).
+
+Lemma good_weaken : forall (A A' : environment -> Prop) e v,
+  (forall Γ, A' Γ -> A Γ) -> good σ S A e v -> good σ S A' e v.
+Proof.
+  intros A A' e v Himp Hg bk be.
+  destruct (Hg bk be) as [h [K H]]. exists h, K.
+  intros Γc Φ Γs e_s k kenv n v_s HA. exact (H Γc Φ Γs e_s k kenv n v_s (Himp Γc HA)).
+Qed.
+
+Lemma thunk_good : forall Γ' e v,
+  good σ S (eq Γ') e v -> good σ S (fun _ => True) (EThunk Γ' e) v.
+Proof.
+  intros Γ' e v Hbody. apply good_at_of_core. intros bk be IH.
+  destruct (Hbody bk bk) as [h0 [K0 H0]].
+  assert (Hprev : exists h1 K1, forall Γc Φ Γs e_s k kenv n v_s,
+    k < bk -> kenv < bk -> σ ⊨ Φ ->
+    contains_env_k σ S kenv Γs Γc -> contains_k σ S k e_s (EThunk Γ' e) ->
+    h1 <= n -> eval (Fin n) Φ Γs e_s v_s ->
+    exists k', k' <= K1 /\ contains_k σ S k' v_s v).
+  { destruct bk as [| bk'].
+    - exists 0, 0. intros. lia.
+    - destruct (IH bk' ltac:(lia) bk') as [h1 [K1 H1]].
+      exists h1, K1. intros Γc0 Φ0 Γs0 e0 k0 ke0 n0 v0 Hk0 Hke0 Hm0 He0 Hc0 Hn0 Hev0.
+      exact (H1 Γc0 Φ0 Γs0 e0 k0 ke0 n0 v0 I ltac:(lia) ltac:(lia) Hm0 He0 Hc0 Hn0 Hev0). }
+  destruct Hprev as [h1 [K1 H1]].
+  exists (1 + h0 + h1), (K0 + K1).
+  intros Γc Φ Γs e_s k kenv n v_s _ Hk Hkenv Hm Henv Hcont Hif Hn Hev.
+  destruct n as [| n]; [lia |].
+  inversion Hcont; subst; try cont_absurd Hif.
+  - inversion Hev; subst; try sym_absurd.
+    change (dec (Remaining n)) with (Fin n) in *.
+    match goal with
+    | [ He : contains_env_k _ _ ?ke ?G Γ', Hb : contains_k _ _ ?kb ?b e,
+        Hv : eval (Fin n) Φ ?G ?b v_s |- _ ] =>
+        destruct (H0 Γ' Φ G b kb ke n v_s eq_refl ltac:(lia) ltac:(lia) Hm He Hb ltac:(lia) Hv)
+          as [k' [Hk' Hc']]
+    end.
+    exists k'. split; [lia | exact Hc'].
+  - inversion Hev; subst; try sym_absurd.
+    change (dec (Remaining n)) with (Fin n) in *.
+    match goal with
+    | [ He : contains_env_k _ _ ?ke ?G ?Gc, Hb : contains_k _ _ ?kb ?b (EThunk Γ' e),
+        Hv : eval (Fin n) Φ ?G ?b v_s |- _ ] =>
+        destruct (H1 Gc Φ G b kb ke n v_s ltac:(lia) ltac:(lia) Hm He Hb ltac:(lia) Hv)
+          as [k' [Hk' Hc']]
+    end.
+    exists k'. split; [lia | exact Hc'].
+Qed.
+
+Lemma con_core : forall Γc0 e_c d args_c bk be,
+  unspool_app e_c [] = (ECon d, args_c) ->
+  core_at σ S (eq Γc0) e_c (make_con_app d (map (delay Γc0) args_c)) bk be.
+Proof.
+  intros Γc0 e_c d args_c bk be Hu.
+  exists 1, (length args_c * (1 + be) + bk).
+  intros Γc Φ Γs e_s k kenv n v_s HA Hk Hkenv Hm Henv Hcont Hif Hn Hev. subst Γc.
+  destruct n as [| n]; [lia |].
+  destruct (contains_k_unspool_rigid_rev σ S k e_s e_c Hcont nil nil nil (ECon d) args_c
+              (Forall3_nil _) Hu eq_refl Hif) as [args_s [ks [Hus [HF Hs]]]].
+  simpl in Hs.
+  assert (Hv : v_s = make_con_app d (map (delay Γs) args_s)).
+  { inversion Hev; subst; sym_absurd. }
+  subst v_s.
+  destruct (delay_map_contains_k σ S kenv Γs Γc0 ks args_s args_c Henv HF) as [ks' [Hks' HF']].
+  exists (0 + list_sum ks'). split.
+  - pose proof (forall3_length_left_right _ _ _ _ _ _ _ HF) as Hlen. rewrite <- Hlen. nia.
+  - unfold make_con_app. exact (contains_k_fold_left_app σ S ks' _ _ 0 _ _ HF' (ContK_Con σ S d)).
+Qed.
+
+Lemma args_good : forall Γc0 args_c args_c',
+  Forall2 (fun a a' => good σ S (eq Γc0) a a') args_c args_c' ->
+  forall bk be, exists h K, forall Φ Γs ks args_s args_s' kenv n,
+    list_sum ks <= bk -> kenv <= be -> σ ⊨ Φ ->
+    contains_env_k σ S kenv Γs Γc0 ->
+    Forall3 (contains_k σ S) ks args_s args_c ->
+    h <= n -> Forall2 (eval (Fin n) Φ Γs) args_s args_s' ->
+    exists ks', Forall3 (contains_k σ S) ks' args_s' args_c' /\ list_sum ks' <= K.
+Proof.
+  intros Γc0 args_c args_c' HG bk be.
+  induction HG as [| a a' l l' Ha _ IH].
+  - exists 0, 0. intros Φ Γs ks args_s args_s' kenv n _ _ _ _ HF _ HE.
+    inversion HF; subst. inversion HE; subst. exists nil. split; [constructor | simpl; lia].
+  - destruct IH as [h1 [K1 H1]]. destruct (Ha bk be) as [h0 [K0 H0]].
+    exists (h0 + h1), (K0 + K1).
+    intros Φ Γs ks args_s args_s' kenv n Hks Hkenv Hm Henv HF Hn HE.
+    inversion HF as [| k0 as0 ac0 ks0 las lac Hc0 HF0]; subst.
+    inversion HE as [| x x' lx lx' Hx HE0]; subst.
+    simpl in Hks.
+    destruct (H0 Γc0 Φ Γs as0 k0 kenv n x' eq_refl ltac:(lia) Hkenv Hm Henv Hc0 ltac:(lia) Hx)
+      as [k' [Hk' Hc']].
+    destruct (H1 Φ Γs ks0 las lx' kenv n ltac:(lia) Hkenv Hm Henv HF0 ltac:(lia) HE0)
+      as [ks' [HF' Hks']].
+    exists (k' :: ks'). split; [constructor; assumption | simpl; lia].
+Qed.
+
+Lemma app_prim_core : forall Γc0 c1 c2 p args_c args_c' bk be,
+  unspool_app (EApp c1 c2) [] = (EPrimOp p, args_c) ->
+  Forall2 (fun a a' => good σ S (eq Γc0) a a') args_c args_c' ->
+  core_at σ S (eq Γc0) (EApp c1 c2) (reduce_prim p args_c') bk be.
+Proof.
+  intros Γc0 c1 c2 p args_c args_c' bk be Hu HG.
+  destruct (args_good Γc0 args_c args_c' HG bk be) as [h0 [K0 H0]].
+  exists (1 + h0), (K0 + prim_slack args_c').
+  intros Γc Φ Γs e_s k kenv n v_s HA Hk Hkenv Hm Henv Hcont Hif Hn Hev. subst Γc.
+  destruct n as [| n]; [lia |].
+  destruct (contains_k_unspool_rigid_rev σ S k e_s _ Hcont nil nil nil (EPrimOp p) args_c
+              (Forall3_nil _) Hu eq_refl Hif) as [args_s [ks [Hus [HF Hs]]]].
+  simpl in Hs.
+  inversion Hev; subst; try sym_absurd.
+  change (dec (Remaining n)) with (Fin n) in *.
+  match goal with [ H2 : unspool_app _ [] = (EPrimOp _, _), HE : Forall2 _ _ ?a' |- _ ] =>
+    rewrite Hus in H2; injection H2 as <- <-;
+    destruct (H0 Φ Γs ks args_s a' kenv n ltac:(lia) Hkenv Hm Henv HF ltac:(lia) HE)
+      as [ks' [HF' Hks']]
+  end.
+  destruct (reduce_prim_contains_k σ S p ks' _ args_c' HF') as [k' [Hk' Hc']].
+  exists k'. split; [lia | exact Hc'].
+Qed.
+
+Lemma app_spine_core : forall Γc0 c1 c2 c1' v bk be,
+  Comp Γc0 c1 ->
+  (forall l, spine_head c1 <> ELit l) ->
+  good σ S (eq Γc0) c1 c1' ->
+  good σ S (eq Γc0) (EApp c1' c2) v ->
+  core_at σ S (eq Γc0) (EApp c1 c2) v bk be.
+Proof.
+  intros Γc0 c1 c2 c1' v bk be Hcomp Hl IH1 IH2.
+  destruct (IH1 bk be) as [h1 [K1 H1]].
+  destruct (IH2 (K1 + bk) be) as [h2 [K2 H2]].
+  exists (1 + h1 + h2), K2.
+  intros Γc Φ Γs e_s k kenv n v_s HA Hk Hkenv Hm Henv Hcont Hif Hn Hev. subst Γc.
+  destruct n as [| n]; [lia |].
+  inversion Hcont; subst; try cont_absurd Hif.
+  match goal with [ Hf : contains_k _ _ ?kf ?f c1, Ha : contains_k _ _ ?ka ?a c2 |- _ ] =>
+    rename Hf into Hfc; rename Ha into Hac; rename f into fs; rename a into as_;
+    rename kf into kfs; rename ka into kas end.
+  assert (Hif' : is_if (spine_head fs) = false).
+  { rewrite (fst_unspool_app _ []) in Hif. simpl in Hif. exact Hif. }
+  pose proof (comp_k_rev σ S kenv kfs Γs Γc0 fs c1 Henv Hfc Hcomp Hif' Hl) as Hcs.
+  inversion Hev; subst; try sym_absurd.
+  change (dec (Remaining n)) with (Fin n) in *.
+  match goal with
+  | [ Hv1 : eval (Fin n) Φ Γs fs ?f', Hv2 : eval (Fin n) Φ Γs (EApp ?f' as_) v_s |- _ ] =>
+      destruct (H1 Γc0 Φ Γs fs kfs kenv n f' eq_refl ltac:(lia) Hkenv Hm Henv Hfc ltac:(lia) Hv1)
+        as [k' [Hk' Hc']];
+      exact (H2 Γc0 Φ Γs (EApp f' as_) (k' + kas) kenv n v_s eq_refl ltac:(lia) Hkenv Hm Henv
+               (ContK_App _ _ _ _ _ _ _ _ Hc' Hac) ltac:(lia) Hv2)
+  end.
+Qed.
+
+End MoreCores.
+
+Section CaseCores.
+Context {sorts : SymCoreSorts} {solver : SymCoreSolver} {laws : SymFCCostLaws}.
+Context (σ : valuation) (S : symvars).
+
+Lemma case_core : forall Γc0 esc altsc esc' v bk be,
+  good σ S (eq Γc0) esc esc' ->
+  fgood σ S (eq Γc0) esc' altsc v ->
+  (inert_scrutinee esc' -> v = EBot BUndefined) ->
+  core_at σ S (eq Γc0) (ECase esc altsc) v bk be.
+Proof.
+  intros Γc0 esc altsc esc' v bk be IH1 IHF Hinert.
+  destruct (IH1 bk be) as [h1 [K1 H1]].
+  destruct (IHF ((1 + field_count esc') * K1) (be + bk)) as [hF [KF HF]].
+  exists (1 + h1 + hF), KF.
+  intros Γc Φ Γs e_s k kenv n v_s HA Hk Hkenv Hm Henv Hcont Hif Hn Hev. subst Γc.
+  destruct n as [| n]; [lia |].
+  inversion Hcont; subst; try cont_absurd Hif.
+  inversion Hev; subst; try sym_absurd.
+  change (dec (Remaining n)) with (Fin n) in *.
+  match goal with
+  | [ Hc : contains_k _ _ ?k1 ?ess esc, Ha : Forall3 _ ?ks ?altss altsc,
+      Hv : eval (Fin n) Φ Γs ?ess ?ess', Hf : fold_alts (Fin n) Φ Γs (merge Γs ?ess') ?altss v_s |- _ ] =>
+      destruct (H1 Γc0 Φ Γs ess k1 kenv n ess' eq_refl ltac:(lia) Hkenv Hm Henv Hc ltac:(lia) Hv)
+        as [k' [Hk' Hc']];
+      destruct (merge_contains_k σ S Γs k' ess' esc' Hc') as [[k'' [Hk'' Hm'']] | [Hi1 Hi2]];
+      [ exact (HF Γc0 Φ Γs (merge Γs ess') altss k'' ks kenv n v_s eq_refl ltac:(nia) ltac:(lia)
+                 ltac:(lia) Hm Henv Hm'' Ha ltac:(lia) Hf)
+      | rewrite (Hinert Hi2), (fold_alts_inert _ _ _ _ _ _ Hi1 Hf);
+        exists 0; split; [lia | apply ContK_Bot] ]
+  end.
+Qed.
+
+Lemma fcon_core : forall Γc0 esc d ea_c xs epc altsc v bk be,
+  decompose_con_app esc = Some (d, ea_c) ->
+  find_alt d altsc = Some (xs, epc) ->
+  Forall concore_expr ea_c ->
+  good σ S (eq (extend_env_multi Γc0 xs ea_c Γc0)) epc v ->
+  fcore_at σ S (eq Γc0) esc altsc v bk be.
+Proof.
+  intros Γc0 esc d ea_c xs epc altsc v bk be Hd Hf Hcon IH.
+  destruct (IH be (be + length xs * (be + bk))) as [h0 [K0 H0]].
+  exists h0, K0.
+  intros Γc Φ Γs m altss k ks kenv n v_s HA Hk Hkenv Hks Hm Henv Hcont Halts Hif Hn Hev. subst Γc.
+  destruct (contains_k_unspool_rigid_rev σ S k m esc Hcont nil nil nil (ECon d) ea_c
+              (Forall3_nil _) (decompose_con_app_unspool esc d ea_c Hd) eq_refl Hif)
+    as [args_s [ks' [Hus [HF Hs]]]].
+  simpl in Hs.
+  destruct (find_alt_contains_alt_k_rev σ S ks altss altsc d xs epc Halts Hf)
+    as [eps [kp [Hfs [Hxs [Hep Hkp]]]]].
+  destruct (extend_env_multi_contains_k σ S xs kenv kenv ks' Γs Γc0 Γs Γc0 args_s ea_c
+              Hxs Henv Henv HF Hcon) as [k' [Hk' Henv']].
+  assert (Hds : decompose_con_app m = Some (d, args_s)) by (unfold decompose_con_app; rewrite Hus; reflexivity).
+  inversion Hev; subst.
+  - simpl in Hif. discriminate Hif.
+  - simpl in Hif. discriminate Hif.
+  - match goal with
+    | [ Hd' : decompose_con_app m = Some _, Hf' : find_alt _ altss = Some _,
+        Hv : eval (Fin n) Φ _ _ v_s |- _ ] =>
+        rewrite Hds in Hd'; injection Hd' as <- <-;
+        rewrite Hfs in Hf'; injection Hf' as <- <-;
+        exact (H0 _ Φ _ eps kp k' n v_s eq_refl ltac:(lia) ltac:(nia) Hm Henv' Hep ltac:(lia) Hv)
+    end.
+  - unfold decompose_con_app in Hds. simpl in Hds. discriminate Hds.
+  - match goal with [ Hmatch : match decompose_con_app m with _ => _ end |- _ ] =>
+      rewrite Hds in Hmatch; congruence end.
+Qed.
+
+Lemma fbot_core : forall Γc0 b altsc bk be,
+  fcore_at σ S (eq Γc0) (EBot b) altsc (EBot b) bk be.
+Proof.
+  intros Γc0 b altsc bk be.
+  exists 0, 0.
+  intros Γc Φ Γs m altss k ks kenv n v_s HA Hk Hkenv Hks Hm Henv Hcont Halts Hif Hn Hev. subst Γc.
+  inversion Hcont; subst; try cont_absurd Hif.
+  inversion Hev; subst.
+  - match goal with [ Hd : decompose_con_app _ = Some _ |- _ ] =>
+      unfold decompose_con_app in Hd; simpl in Hd; discriminate Hd end.
+  - exists 0. split; [lia | apply ContK_Bot].
+  - match goal with [ Hb : is_bot _ = false |- _ ] => simpl in Hb; discriminate Hb end.
+Qed.
+
+Lemma fotherwise_core : forall Γc0 esc altsc bk be,
+  (match decompose_con_app esc with
+   | Some (d, _) => find_alt d altsc = None
+   | None => True
+   end) ->
+  is_bot esc = false ->
+  fcore_at σ S (eq Γc0) esc altsc (EBot BUndefined) bk be.
+Proof.
+  intros Γc0 esc altsc bk be Hmatch Hbot.
+  exists 0, 0.
+  intros Γc Φ Γs m altss k ks kenv n v_s HA Hk Hkenv Hks Hm Henv Hcont Halts Hif Hn Hev. subst Γc.
+  inversion Hev; subst.
+  - simpl in Hif. discriminate Hif.
+  - simpl in Hif. discriminate Hif.
+  - exfalso.
+    match goal with
+    | [ Hd : decompose_con_app m = Some (?d, ?ea), Hf : find_alt ?d altss = Some (?xs, ?ep) |- _ ] =>
+        destruct (contains_k_unspool_con σ S k m esc Hcont nil nil nil (Forall3_nil _) d ea
+                    (decompose_con_app_unspool m d ea Hd)) as [args_c [ks' [Huc _]]];
+        assert (Hdc : decompose_con_app esc = Some (d, args_c))
+          by (unfold decompose_con_app; simpl in Huc; rewrite Huc; reflexivity);
+        rewrite Hdc in Hmatch;
+        destruct (find_alt_contains_alt σ S altss altsc d xs ep
+                    (contains_alts_k_erase σ S ks altss altsc Halts) Hf) as [epc [Hfc _]];
+        congruence
+    end.
+  - exfalso. inversion Hcont; subst; try cont_absurd Hif. simpl in Hbot. discriminate Hbot.
+  - exists 0. split; [lia | apply ContK_Bot].
+Qed.
+
+End CaseCores.
+
+Section Main.
+Context {sorts : SymCoreSorts} {solver : SymCoreSolver} {laws : SymFCCostLaws}.
+Context (σ : valuation) (S : symvars).
+
+Definition eval_motive (f : fuel) (Φ : path_condition) (Γ : environment) (e v : expr) : Prop :=
+  f = Inf -> Φ = pc_true -> concore_expr e -> concrete_env Γ -> good σ S (eq Γ) e v.
+
+Definition fold_motive (f : fuel) (Φ : path_condition) (Γ : environment) (e : expr)
+  (alts : list alt) (v : expr) : Prop :=
+  f = Inf -> Φ = pc_true -> concore_expr e -> Forall concore_alt alts -> concrete_env Γ ->
+  fgood σ S (eq Γ) e alts v.
+
+Lemma forall2_good_of_ind : forall Γ args args',
+  Forall2 (fun a a' => eval Inf pc_true Γ a a' /\ eval_motive Inf pc_true Γ a a') args args' ->
+  Forall concore_expr args -> concrete_env Γ ->
+  Forall2 (fun a a' => good σ S (eq Γ) a a') args args'.
+Proof.
+  intros Γ args args' HF Hc Hg. induction HF as [| a a' l l' [_ Ha] _ IH]; constructor.
+  - inversion Hc; subst. exact (Ha eq_refl eq_refl ltac:(assumption) Hg).
+  - inversion Hc; subst. exact (IH ltac:(assumption)).
+Qed.
+
+Theorem concrete_good : forall Γc e_c v_c,
+  eval Inf pc_true Γc e_c v_c -> concore_expr e_c -> concrete_env Γc ->
+  good σ S (eq Γc) e_c v_c.
+Proof.
+  intros Γc e_c v_c H.
+  refine (eval_nested_ind eval_motive fold_motive _ _ _ _ _ _ _ _ _ _ _ _ _ _ _ _ _ _ _ _
+            _ _ _ _ _ Inf pc_true Γc e_c v_c H eq_refl eq_refl);
+    unfold eval_motive, fold_motive.
+  - intros f Φ Γ x Γ' e e' Hl _ IH Hf HΦ Hc Hg. injection Hf as ->. subst Φ.
+    destruct (lookup_env_concrete Γ x Γ' e Hg Hl) as [Hg' He].
+    apply good_at_of_core. intros bk be _.
+    exact (var_core σ S Γ x Γ' e e' bk be Hl (IH eq_refl eq_refl He Hg')).
+  - intros f Φ Γ x Hl _ _ _ _. apply good_at_of_core. intros bk be _.
+    exact (symvar_core σ S Γ x bk be Hl).
+  - intros f Φ Γ l _ _ _ _. apply good_at_of_core. intros bk be _. apply lit_core.
+  - intros f Φ Γ e d args Hu _ _ _ _. apply good_at_of_core. intros bk be _.
+    exact (con_core σ S Γ e d args bk be Hu).
+  - intros f Φ Γ e γ e' _ IH Hf HΦ Hc Hg. injection Hf as ->. subst Φ.
+    apply good_at_of_core. intros bk be _.
+    exact (cast_core σ S Γ e γ e' bk be (IH eq_refl eq_refl (concore_expr_cast e γ Hc) Hg)).
+  - intros f Φ Γ Γ' x eb ea eb' _ IH Hf HΦ Hc Hg. injection Hf as ->. subst Φ.
+    pose proof (concore_expr_app_l _ _ Hc) as Hcf.
+    pose proof (concore_expr_app_r _ _ Hc) as Hca.
+    pose proof (concore_expr_lam _ _ (concore_expr_thunk _ _ Hcf)) as Hcb.
+    pose proof (concore_expr_thunk_env _ _ Hcf) as Hg'.
+    apply good_at_of_core. intros bk be _.
+    exact (app_abs_core σ S Γ Γ' x eb ea eb'
+             (IH eq_refl eq_refl Hcb (concrete_env_extend Γ' x Γ ea Hg' Hg Hca)) Hca bk be).
+  - intros f Φ Γ ef ea ef' er Hcomp Hev1 IH1 _ IH2 Hf HΦ Hc Hg. injection Hf as ->. subst Φ.
+    pose proof (concore_expr_app_l _ _ Hc) as Hcf.
+    pose proof (concore_expr_app_r _ _ Hc) as Hca.
+    pose proof (concore_eval_closed Γ ef ef' Hg Hcf Hev1) as Hcf'.
+    assert (Hl : forall l, spine_head ef <> ELit l).
+    { intros l Hsh. pose proof (eval_spine_head_lit _ _ _ _ _ Hev1 eq_refl eq_refl l Hsh) as ->.
+      inversion Hcomp. }
+    apply good_at_of_core. intros bk be _.
+    exact (app_spine_core σ S Γ ef ea ef' er bk be Hcomp Hl (IH1 eq_refl eq_refl Hcf Hg)
+             (IH2 eq_refl eq_refl (Con_App _ _ Hcf' Hca) Hg)).
+  - intros f Φ Γ b _ _ _ _. apply good_at_of_core. intros bk be _. apply bot_core.
+  - intros f Φ Γ ef ea p args args' Hu _ HF Hf HΦ Hc Hg. injection Hf as ->. subst Φ.
+    destruct (unspool_app_concore _ _ _ _ Hu Hc (Forall_nil _)) as [_ Hargs].
+    apply good_at_of_core. intros bk be _.
+    exact (app_prim_core σ S Γ ef ea p args args' bk be Hu (forall2_good_of_ind Γ args args' HF Hargs Hg)).
+  - intros f Φ Γ x e _ _ _ _. apply good_at_of_core. intros bk be _. apply lam_core.
+  - intros f Φ Γ ef γ ea γ_a γ_r er Hd _ IH Hf HΦ Hc Hg. injection Hf as ->. subst Φ.
+    pose proof (concore_expr_app_l _ _ Hc) as Hcf.
+    pose proof (concore_expr_app_r _ _ Hc) as Hca.
+    pose proof (concore_expr_cast _ _ Hcf) as Hcf0.
+    apply good_at_of_core. intros bk be _.
+    exact (app_cast_core σ S Γ ef γ ea γ_a γ_r er bk be Hd
+             (IH eq_refl eq_refl (Con_Cast _ _ (Con_App _ _ Hcf0 (Con_Cast _ _ Hca))) Hg)).
+  - intros f Φ Γ e1 e2 ec et ef args er Hu _ _ _ _ Hc _. exfalso.
+    destruct (unspool_app_concore _ _ _ _ Hu Hc (Forall_nil _)) as [Hh _].
+    exact (not_concore_if _ _ _ Hh).
+  - intros f Φ Γ b ea _ _ _ _. apply good_at_of_core. intros bk be _. apply app_bot_core.
+  - intros f Φ Γ es alts es' er Hev1 IH1 Hfold IHF Hf HΦ Hc Hg. injection Hf as ->. subst Φ.
+    inversion Hc as [| | | | | | es0 alts0 Hces Halts | | | | | | |]; subst.
+    pose proof (concore_eval_closed Γ es es' Hg Hces Hev1) as Hces'.
+    change (dec Unlimited) with Inf in *.
+    rewrite (merge_concore_id Γ es' Hces') in Hfold, IHF.
+    apply good_at_of_core. intros bk be _.
+    exact (case_core σ S Γ es alts es' er bk be (IH1 eq_refl eq_refl Hces Hg)
+             (IHF eq_refl eq_refl Hces' Halts Hg) (fun Hi => fold_alts_inert _ _ _ _ _ _ Hi Hfold)).
+  - intros. exfalso. match goal with [ Hc : concore_expr (EIf _ _ _) |- _ ] =>
+      exact (not_concore_if _ _ _ Hc) end.
+  - intros f Φ Γ γ _ _ _ _. apply good_at_of_core. intros bk be _. apply coercion_core.
+  - intros f Φ Γ e Hs _ HΦ _ _. subst Φ. rewrite sat_pc_true in Hs. discriminate Hs.
+  - intros f Φ Γ τ _ _ _ _. apply good_at_of_core. intros bk be _. apply type_core.
+  - intros f Φ Γ Γ' e e' _ IH Hf HΦ Hc Hg. injection Hf as ->. subst Φ.
+    apply (good_weaken σ S (fun _ => True)); [intros; exact I |].
+    apply thunk_good.
+    exact (IH eq_refl eq_refl (concore_expr_thunk _ _ Hc) (concore_expr_thunk_env _ _ Hc)).
+  - intros Φ Γ e Hf. discriminate Hf.
+  - intros. exfalso. match goal with [ Hc : concore_expr (EIf _ _ _) |- _ ] =>
+      exact (not_concore_if _ _ _ Hc) end.
+  - intros. exfalso. match goal with [ Hc : concore_expr (EIf _ _ _) |- _ ] =>
+      exact (not_concore_if _ _ _ Hc) end.
+  - intros f Φ Γ e d ea xs ep alts er Hd Hfa _ IH Hf HΦ Hc Halts Hg. subst f Φ.
+    pose proof (decompose_con_app_concore e d ea Hd Hc) as Hea.
+    pose proof (find_alt_concore d alts xs ep Hfa Halts) as Hep.
+    apply fgood_of_core. intros bk be _.
+    exact (fcon_core σ S Γ e d ea xs ep alts er bk be Hd Hfa Hea
+             (IH eq_refl eq_refl Hep (concrete_env_extend_multi xs ea Γ Γ Hg Hg Hea))).
+  - intros f Φ Γ b alts _ _ _ _ _. apply fgood_of_core. intros bk be _. apply fbot_core.
+  - intros f Φ Γ e alts _ Hmatch Hbot _ _ _ _ _. apply fgood_of_core. intros bk be _.
+    exact (fotherwise_core σ S Γ e alts bk be Hmatch Hbot).
+Qed.
+
+Theorem forall_form : forall Γc e_con v_con,
+  Γc ⊢ᶜ e_con ⇓ᶜ v_con ->
+  forall Φ Γs e_sym,
+    σ ⊨ Φ ->
+    contains_env σ S Γs Γc ->
+    contains σ S e_sym e_con ->
+    concore_expr e_con ->
+    exists h, forall n, (h <= n)%nat ->
+      forall v_sym, eval (Fin n) Φ Γs e_sym v_sym -> contains σ S v_sym v_con.
+Proof.
+  intros Γc e_con v_con Hevc Φ Γs e_sym Hm Henv Hcont Hcon.
+  destruct (contains_k_of_contains _ _ _ _ Hcont) as [k Hk].
+  destruct (contains_env_k_of_contains_env _ _ _ _ Henv) as [kenv Hkenv].
+  destruct (concrete_good Γc e_con v_con Hevc Hcon (contains_env_concrete σ S Γs Γc Henv)
+              (k + kenv) (k + kenv)) as [h [K H]].
+  exists h. intros n Hn v_sym Hv.
+  destruct (H Γc Φ Γs e_sym k kenv n v_sym eq_refl ltac:(lia) ltac:(lia) Hm Hkenv Hk Hn Hv)
+    as [k' [_ Hc']].
+  exact (contains_k_erase _ _ _ _ _ Hc').
+Qed.
+
+End Main.
+
+Section CompletenessUnderCostLaws.
+Context {sorts : SymCoreSorts} {solver : SymCoreSolver} {laws : SymFCCostLaws}.
+
+Theorem concore_completeness_forall : forall_form_lemma.
+Proof.
+  intros Γc e_con v_con Hevc Φ Γs σ S e_sym Hm Henv Hcont Hcon.
+  exact (forall_form σ S Γc e_con v_con Hevc Φ Γs e_sym Hm Henv Hcont Hcon).
+Qed.
+
+Theorem concore_completeness_budget : target_completeness.
+Proof.
+  intros Φ Γs Γc σ S e_sym e_con v_con Hm Henv Hcont Hcon [hb Hb] Hevc.
+  destruct (forall_form σ S Γc e_con v_con Hevc Φ Γs e_sym Hm Henv Hcont Hcon) as [h Hh].
+  exists (h + hb). intros n Hn.
+  destruct (Hb n ltac:(lia)) as [v Hv].
+  exists v. split; [exact Hv | exact (Hh n ltac:(lia) v Hv)].
+Qed.
+
+Corollary concore_completeness_exists : existential_corollary.
+Proof. exact (existential_corollary_of_target concore_completeness_budget). Qed.
+
+End CompletenessUnderCostLaws.
